Still cleaning proofs. Replaced some metis/meson by simp add.

src/Operational.thy
@@ -3,154 +3,182 @@ text\<open>\label{chap:operational_semantics}\<close>
 
 theory Operational
 imports
-    "SymbolicPrimitive"
+  SymbolicPrimitive
 
 begin
 
 section\<open>Operational steps\<close>
 
 abbreviation uncurry_conf
-  :: "('\<tau>::linordered_field) system \<Rightarrow> instant_index \<Rightarrow> '\<tau> TESL_formula \<Rightarrow> '\<tau> TESL_formula \<Rightarrow> '\<tau> config" ("_, _ \<turnstile> _ \<triangleright> _" 80) where
-  "\<Gamma>, n \<turnstile> \<Psi> \<triangleright> \<Phi> \<equiv> (\<Gamma>, n, \<Psi>, \<Phi>)"
+  ::\<open>('\<tau>::linordered_field) system \<Rightarrow> instant_index \<Rightarrow> '\<tau> TESL_formula \<Rightarrow> '\<tau> TESL_formula
+      \<Rightarrow> '\<tau> config\<close>                                                  ("_, _ \<turnstile> _ \<triangleright> _" 80)
+where
+  \<open>\<Gamma>, n \<turnstile> \<Psi> \<triangleright> \<Phi> \<equiv> (\<Gamma>, n, \<Psi>, \<Phi>)\<close>
 
-inductive operational_semantics_intro :: "('\<tau>::linordered_field) config \<Rightarrow> '\<tau> config \<Rightarrow> bool" ("_ \<hookrightarrow>\<^sub>i _" 70) where
+inductive operational_semantics_intro
+  ::\<open>('\<tau>::linordered_field) config \<Rightarrow> '\<tau> config \<Rightarrow> bool\<close>              ("_ \<hookrightarrow>\<^sub>i _" 70)
+where
   instant_i:
-  "(\<Gamma>, n \<turnstile> [] \<triangleright> \<Phi>)
-     \<hookrightarrow>\<^sub>i  (\<Gamma>, Suc n \<turnstile> \<Phi> \<triangleright> [])"
+  \<open>(\<Gamma>, n \<turnstile> [] \<triangleright> \<Phi>) \<hookrightarrow>\<^sub>i  (\<Gamma>, Suc n \<turnstile> \<Phi> \<triangleright> [])\<close>
 
-inductive operational_semantics_elim :: "('\<tau>::linordered_field) config \<Rightarrow> '\<tau> config \<Rightarrow> bool" ("_ \<hookrightarrow>\<^sub>e _" 70) where
+inductive operational_semantics_elim
+  ::\<open>('\<tau>::linordered_field) config \<Rightarrow> '\<tau> config \<Rightarrow> bool\<close>              ("_ \<hookrightarrow>\<^sub>e _" 70)
+where
   sporadic_on_e1:
-  "(\<Gamma>, n \<turnstile> ((K\<^sub>1 sporadic \<tau> on K\<^sub>2) # \<Psi>) \<triangleright> \<Phi>)
-     \<hookrightarrow>\<^sub>e  (\<Gamma>, n \<turnstile> \<Psi> \<triangleright> ((K\<^sub>1 sporadic \<tau> on K\<^sub>2) # \<Phi>))"
+  \<open>(\<Gamma>, n \<turnstile> ((K\<^sub>1 sporadic \<tau> on K\<^sub>2) # \<Psi>) \<triangleright> \<Phi>)
+     \<hookrightarrow>\<^sub>e  (\<Gamma>, n \<turnstile> \<Psi> \<triangleright> ((K\<^sub>1 sporadic \<tau> on K\<^sub>2) # \<Phi>))\<close>
 | sporadic_on_e2:
-  "(\<Gamma>, n \<turnstile> ((K\<^sub>1 sporadic \<tau> on K\<^sub>2) # \<Psi>) \<triangleright> \<Phi>)
-     \<hookrightarrow>\<^sub>e  (((K\<^sub>1 \<Up> n) # (K\<^sub>2 \<Down> n @ \<tau>) # \<Gamma>), n \<turnstile> \<Psi> \<triangleright> \<Phi>)"
+  \<open>(\<Gamma>, n \<turnstile> ((K\<^sub>1 sporadic \<tau> on K\<^sub>2) # \<Psi>) \<triangleright> \<Phi>)
+     \<hookrightarrow>\<^sub>e  (((K\<^sub>1 \<Up> n) # (K\<^sub>2 \<Down> n @ \<tau>) # \<Gamma>), n \<turnstile> \<Psi> \<triangleright> \<Phi>)\<close>
 | tagrel_e:
-  "(\<Gamma>, n \<turnstile> ((time-relation \<lfloor>K\<^sub>1, K\<^sub>2\<rfloor> \<in> R) # \<Psi>) \<triangleright> \<Phi>)
-     \<hookrightarrow>\<^sub>e  (((\<lfloor>\<tau>\<^sub>v\<^sub>a\<^sub>r(K\<^sub>1, n), \<tau>\<^sub>v\<^sub>a\<^sub>r(K\<^sub>2, n)\<rfloor> \<in> R) # \<Gamma>), n \<turnstile> \<Psi> \<triangleright> ((time-relation \<lfloor>K\<^sub>1, K\<^sub>2\<rfloor> \<in> R) # \<Phi>))"
+  \<open>(\<Gamma>, n \<turnstile> ((time-relation \<lfloor>K\<^sub>1, K\<^sub>2\<rfloor> \<in> R) # \<Psi>) \<triangleright> \<Phi>)
+     \<hookrightarrow>\<^sub>e  (((\<lfloor>\<tau>\<^sub>v\<^sub>a\<^sub>r(K\<^sub>1, n), \<tau>\<^sub>v\<^sub>a\<^sub>r(K\<^sub>2, n)\<rfloor> \<in> R) # \<Gamma>), n \<turnstile> \<Psi> \<triangleright> ((time-relation \<lfloor>K\<^sub>1, K\<^sub>2\<rfloor> \<in> R) # \<Phi>))\<close>
 | implies_e1:
-  "(\<Gamma>, n \<turnstile> ((K\<^sub>1 implies K\<^sub>2) # \<Psi>) \<triangleright> \<Phi>)
-     \<hookrightarrow>\<^sub>e  (((K\<^sub>1 \<not>\<Up> n) # \<Gamma>), n \<turnstile> \<Psi> \<triangleright> ((K\<^sub>1 implies K\<^sub>2) # \<Phi>))"
+  \<open>(\<Gamma>, n \<turnstile> ((K\<^sub>1 implies K\<^sub>2) # \<Psi>) \<triangleright> \<Phi>)
+     \<hookrightarrow>\<^sub>e  (((K\<^sub>1 \<not>\<Up> n) # \<Gamma>), n \<turnstile> \<Psi> \<triangleright> ((K\<^sub>1 implies K\<^sub>2) # \<Phi>))\<close>
 | implies_e2:
-  "(\<Gamma>, n \<turnstile> ((K\<^sub>1 implies K\<^sub>2) # \<Psi>) \<triangleright> \<Phi>)
-     \<hookrightarrow>\<^sub>e  (((K\<^sub>1 \<Up> n) # (K\<^sub>2 \<Up> n) # \<Gamma>), n \<turnstile> \<Psi> \<triangleright> ((K\<^sub>1 implies K\<^sub>2) # \<Phi>))"
+  \<open>(\<Gamma>, n \<turnstile> ((K\<^sub>1 implies K\<^sub>2) # \<Psi>) \<triangleright> \<Phi>)
+     \<hookrightarrow>\<^sub>e  (((K\<^sub>1 \<Up> n) # (K\<^sub>2 \<Up> n) # \<Gamma>), n \<turnstile> \<Psi> \<triangleright> ((K\<^sub>1 implies K\<^sub>2) # \<Phi>))\<close>
 | implies_not_e1:
-  "(\<Gamma>, n \<turnstile> ((K\<^sub>1 implies not K\<^sub>2) # \<Psi>) \<triangleright> \<Phi>)
-     \<hookrightarrow>\<^sub>e  (((K\<^sub>1 \<not>\<Up> n) # \<Gamma>), n \<turnstile> \<Psi> \<triangleright> ((K\<^sub>1 implies not K\<^sub>2) # \<Phi>))"
+  \<open>(\<Gamma>, n \<turnstile> ((K\<^sub>1 implies not K\<^sub>2) # \<Psi>) \<triangleright> \<Phi>)
+     \<hookrightarrow>\<^sub>e  (((K\<^sub>1 \<not>\<Up> n) # \<Gamma>), n \<turnstile> \<Psi> \<triangleright> ((K\<^sub>1 implies not K\<^sub>2) # \<Phi>))\<close>
 | implies_not_e2:
-  "(\<Gamma>, n \<turnstile> ((K\<^sub>1 implies not K\<^sub>2) # \<Psi>) \<triangleright> \<Phi>)
-     \<hookrightarrow>\<^sub>e  (((K\<^sub>1 \<Up> n) # (K\<^sub>2 \<not>\<Up> n) # \<Gamma>), n \<turnstile> \<Psi> \<triangleright> ((K\<^sub>1 implies not K\<^sub>2) # \<Phi>))"
+  \<open>(\<Gamma>, n \<turnstile> ((K\<^sub>1 implies not K\<^sub>2) # \<Psi>) \<triangleright> \<Phi>)
+     \<hookrightarrow>\<^sub>e  (((K\<^sub>1 \<Up> n) # (K\<^sub>2 \<not>\<Up> n) # \<Gamma>), n \<turnstile> \<Psi> \<triangleright> ((K\<^sub>1 implies not K\<^sub>2) # \<Phi>))\<close>
 | timedelayed_e1:
-  "(\<Gamma>, n \<turnstile> ((K\<^sub>1 time-delayed by \<delta>\<tau> on K\<^sub>2 implies K\<^sub>3) # \<Psi>) \<triangleright> \<Phi>)
-     \<hookrightarrow>\<^sub>e  (((K\<^sub>1 \<not>\<Up> n) # \<Gamma>), n \<turnstile> \<Psi> \<triangleright> ((K\<^sub>1 time-delayed by \<delta>\<tau> on K\<^sub>2 implies K\<^sub>3) # \<Phi>))"
+  \<open>(\<Gamma>, n \<turnstile> ((K\<^sub>1 time-delayed by \<delta>\<tau> on K\<^sub>2 implies K\<^sub>3) # \<Psi>) \<triangleright> \<Phi>)
+     \<hookrightarrow>\<^sub>e  (((K\<^sub>1 \<not>\<Up> n) # \<Gamma>), n \<turnstile> \<Psi> \<triangleright> ((K\<^sub>1 time-delayed by \<delta>\<tau> on K\<^sub>2 implies K\<^sub>3) # \<Phi>))\<close>
 | timedelayed_e2:
-  "(\<Gamma>, n \<turnstile> ((K\<^sub>1 time-delayed by \<delta>\<tau> on K\<^sub>2 implies K\<^sub>3) # \<Psi>) \<triangleright> \<Phi>)
-     \<hookrightarrow>\<^sub>e  (((K\<^sub>1 \<Up> n) # (K\<^sub>2 @ n \<oplus> \<delta>\<tau> \<Rightarrow> K\<^sub>3) # \<Gamma>), n \<turnstile> \<Psi> \<triangleright> ((K\<^sub>1 time-delayed by \<delta>\<tau> on K\<^sub>2 implies K\<^sub>3) # \<Phi>))"
+  \<open>(\<Gamma>, n \<turnstile> ((K\<^sub>1 time-delayed by \<delta>\<tau> on K\<^sub>2 implies K\<^sub>3) # \<Psi>) \<triangleright> \<Phi>)
+     \<hookrightarrow>\<^sub>e  (((K\<^sub>1 \<Up> n) # (K\<^sub>2 @ n \<oplus> \<delta>\<tau> \<Rightarrow> K\<^sub>3) # \<Gamma>), n
+            \<turnstile> \<Psi> \<triangleright> ((K\<^sub>1 time-delayed by \<delta>\<tau> on K\<^sub>2 implies K\<^sub>3) # \<Phi>))\<close>
 | weakly_precedes_e:
-  "(\<Gamma>, n \<turnstile> ((K\<^sub>1 weakly precedes K\<^sub>2) # \<Psi>) \<triangleright> \<Phi>)
-     \<hookrightarrow>\<^sub>e  (((\<lceil>#\<^sup>\<le> K\<^sub>2 n, #\<^sup>\<le> K\<^sub>1 n\<rceil> \<in> (\<lambda>(x,y). x\<le>y)) # \<Gamma>), n \<turnstile> \<Psi> \<triangleright> ((K\<^sub>1 weakly precedes K\<^sub>2) # \<Phi>))"
+  \<open>(\<Gamma>, n \<turnstile> ((K\<^sub>1 weakly precedes K\<^sub>2) # \<Psi>) \<triangleright> \<Phi>)
+     \<hookrightarrow>\<^sub>e  (((\<lceil>#\<^sup>\<le> K\<^sub>2 n, #\<^sup>\<le> K\<^sub>1 n\<rceil> \<in> (\<lambda>(x,y). x\<le>y)) # \<Gamma>), n
+            \<turnstile> \<Psi> \<triangleright> ((K\<^sub>1 weakly precedes K\<^sub>2) # \<Phi>))\<close>
 | strictly_precedes_e:
-  "(\<Gamma>, n \<turnstile> ((K\<^sub>1 strictly precedes K\<^sub>2) # \<Psi>) \<triangleright> \<Phi>)
-     \<hookrightarrow>\<^sub>e  (((\<lceil>#\<^sup>\<le> K\<^sub>2 n, #\<^sup>< K\<^sub>1 n\<rceil> \<in> (\<lambda>(x,y). x\<le>y)) # \<Gamma>), n \<turnstile> \<Psi> \<triangleright> ((K\<^sub>1 strictly precedes K\<^sub>2) # \<Phi>))"
+  \<open>(\<Gamma>, n \<turnstile> ((K\<^sub>1 strictly precedes K\<^sub>2) # \<Psi>) \<triangleright> \<Phi>)
+     \<hookrightarrow>\<^sub>e  (((\<lceil>#\<^sup>\<le> K\<^sub>2 n, #\<^sup>< K\<^sub>1 n\<rceil> \<in> (\<lambda>(x,y). x\<le>y)) # \<Gamma>), n
+            \<turnstile> \<Psi> \<triangleright> ((K\<^sub>1 strictly precedes K\<^sub>2) # \<Phi>))\<close>
 | kills_e1:
-  "(\<Gamma>, n \<turnstile> ((K\<^sub>1 kills K\<^sub>2) # \<Psi>) \<triangleright> \<Phi>)
-     \<hookrightarrow>\<^sub>e  (((K\<^sub>1 \<not>\<Up> n) # \<Gamma>), n \<turnstile> \<Psi> \<triangleright> ((K\<^sub>1 kills K\<^sub>2) # \<Phi>))"
+  \<open>(\<Gamma>, n \<turnstile> ((K\<^sub>1 kills K\<^sub>2) # \<Psi>) \<triangleright> \<Phi>)
+     \<hookrightarrow>\<^sub>e  (((K\<^sub>1 \<not>\<Up> n) # \<Gamma>), n \<turnstile> \<Psi> \<triangleright> ((K\<^sub>1 kills K\<^sub>2) # \<Phi>))\<close>
 | kills_e2:
-  "(\<Gamma>, n \<turnstile> ((K\<^sub>1 kills K\<^sub>2) # \<Psi>) \<triangleright> \<Phi>)
-     \<hookrightarrow>\<^sub>e  (((K\<^sub>1 \<Up> n) # (K\<^sub>2 \<not>\<Up> \<ge> n) # \<Gamma>), n \<turnstile> \<Psi> \<triangleright> ((K\<^sub>1 kills K\<^sub>2) # \<Phi>))"
+  \<open>(\<Gamma>, n \<turnstile> ((K\<^sub>1 kills K\<^sub>2) # \<Psi>) \<triangleright> \<Phi>)
+     \<hookrightarrow>\<^sub>e  (((K\<^sub>1 \<Up> n) # (K\<^sub>2 \<not>\<Up> \<ge> n) # \<Gamma>), n \<turnstile> \<Psi> \<triangleright> ((K\<^sub>1 kills K\<^sub>2) # \<Phi>))\<close>
 
-inductive operational_semantics_step :: "('\<tau>::linordered_field) config \<Rightarrow> '\<tau> config \<Rightarrow> bool" ("_ \<hookrightarrow> _" 70) where
-    intro_part: "(\<Gamma>\<^sub>1, n\<^sub>1 \<turnstile> \<Psi>\<^sub>1 \<triangleright> \<Phi>\<^sub>1)  \<hookrightarrow>\<^sub>i  (\<Gamma>\<^sub>2, n\<^sub>2 \<turnstile> \<Psi>\<^sub>2 \<triangleright> \<Phi>\<^sub>2)
-   \<Longrightarrow> (\<Gamma>\<^sub>1, n\<^sub>1 \<turnstile> \<Psi>\<^sub>1 \<triangleright> \<Phi>\<^sub>1)  \<hookrightarrow>  (\<Gamma>\<^sub>2, n\<^sub>2 \<turnstile> \<Psi>\<^sub>2 \<triangleright> \<Phi>\<^sub>2)"
-  | elims_part: "(\<Gamma>\<^sub>1, n\<^sub>1 \<turnstile> \<Psi>\<^sub>1 \<triangleright> \<Phi>\<^sub>1)  \<hookrightarrow>\<^sub>e  (\<Gamma>\<^sub>2, n\<^sub>2 \<turnstile> \<Psi>\<^sub>2 \<triangleright> \<Phi>\<^sub>2)
-   \<Longrightarrow> (\<Gamma>\<^sub>1, n\<^sub>1 \<turnstile> \<Psi>\<^sub>1 \<triangleright> \<Phi>\<^sub>1)  \<hookrightarrow>  (\<Gamma>\<^sub>2, n\<^sub>2 \<turnstile> \<Psi>\<^sub>2 \<triangleright> \<Phi>\<^sub>2)"
+inductive operational_semantics_step
+  ::\<open>('\<tau>::linordered_field) config \<Rightarrow> '\<tau> config \<Rightarrow> bool\<close>                ("_ \<hookrightarrow> _" 70)
+where
+  intro_part:
+  \<open>(\<Gamma>\<^sub>1, n\<^sub>1 \<turnstile> \<Psi>\<^sub>1 \<triangleright> \<Phi>\<^sub>1)  \<hookrightarrow>\<^sub>i  (\<Gamma>\<^sub>2, n\<^sub>2 \<turnstile> \<Psi>\<^sub>2 \<triangleright> \<Phi>\<^sub>2)
+    \<Longrightarrow> (\<Gamma>\<^sub>1, n\<^sub>1 \<turnstile> \<Psi>\<^sub>1 \<triangleright> \<Phi>\<^sub>1)  \<hookrightarrow>  (\<Gamma>\<^sub>2, n\<^sub>2 \<turnstile> \<Psi>\<^sub>2 \<triangleright> \<Phi>\<^sub>2)\<close>
+| elims_part:
+  \<open>(\<Gamma>\<^sub>1, n\<^sub>1 \<turnstile> \<Psi>\<^sub>1 \<triangleright> \<Phi>\<^sub>1)  \<hookrightarrow>\<^sub>e  (\<Gamma>\<^sub>2, n\<^sub>2 \<turnstile> \<Psi>\<^sub>2 \<triangleright> \<Phi>\<^sub>2)
+    \<Longrightarrow> (\<Gamma>\<^sub>1, n\<^sub>1 \<turnstile> \<Psi>\<^sub>1 \<triangleright> \<Phi>\<^sub>1)  \<hookrightarrow>  (\<Gamma>\<^sub>2, n\<^sub>2 \<turnstile> \<Psi>\<^sub>2 \<triangleright> \<Phi>\<^sub>2)\<close>
 
-abbreviation operational_semantics_step_rtranclp :: "('\<tau>::linordered_field) config \<Rightarrow> '\<tau> config \<Rightarrow> bool" ("_ \<hookrightarrow>\<^sup>*\<^sup>* _" 70) where
-  "\<C>\<^sub>1 \<hookrightarrow>\<^sup>*\<^sup>* \<C>\<^sub>2 \<equiv> operational_semantics_step\<^sup>*\<^sup>* \<C>\<^sub>1 \<C>\<^sub>2"
+abbreviation operational_semantics_step_rtranclp
+  ::\<open>('\<tau>::linordered_field) config \<Rightarrow> '\<tau> config \<Rightarrow> bool\<close>                ("_ \<hookrightarrow>\<^sup>*\<^sup>* _" 70)
+where
+  \<open>\<C>\<^sub>1 \<hookrightarrow>\<^sup>*\<^sup>* \<C>\<^sub>2 \<equiv> operational_semantics_step\<^sup>*\<^sup>* \<C>\<^sub>1 \<C>\<^sub>2\<close>
 
-abbreviation operational_semantics_step_tranclp :: "('\<tau>::linordered_field) config \<Rightarrow> '\<tau> config \<Rightarrow> bool" ("_ \<hookrightarrow>\<^sup>+\<^sup>+ _" 70) where
-  "\<C>\<^sub>1 \<hookrightarrow>\<^sup>+\<^sup>+ \<C>\<^sub>2 \<equiv> operational_semantics_step\<^sup>+\<^sup>+ \<C>\<^sub>1 \<C>\<^sub>2"
+abbreviation operational_semantics_step_tranclp
+  ::\<open>('\<tau>::linordered_field) config \<Rightarrow> '\<tau> config \<Rightarrow> bool\<close>                ("_ \<hookrightarrow>\<^sup>+\<^sup>+ _" 70)
+where
+  \<open>\<C>\<^sub>1 \<hookrightarrow>\<^sup>+\<^sup>+ \<C>\<^sub>2 \<equiv> operational_semantics_step\<^sup>+\<^sup>+ \<C>\<^sub>1 \<C>\<^sub>2\<close>
 
-abbreviation operational_semantics_step_reflclp :: "('\<tau>::linordered_field) config \<Rightarrow> '\<tau> config \<Rightarrow> bool" ("_ \<hookrightarrow>\<^sup>=\<^sup>= _" 70) where
-  "\<C>\<^sub>1 \<hookrightarrow>\<^sup>=\<^sup>= \<C>\<^sub>2 \<equiv> operational_semantics_step\<^sup>=\<^sup>= \<C>\<^sub>1 \<C>\<^sub>2"
+abbreviation operational_semantics_step_reflclp
+  ::\<open>('\<tau>::linordered_field) config \<Rightarrow> '\<tau> config \<Rightarrow> bool\<close>                ("_ \<hookrightarrow>\<^sup>=\<^sup>= _" 70)
+where
+  \<open>\<C>\<^sub>1 \<hookrightarrow>\<^sup>=\<^sup>= \<C>\<^sub>2 \<equiv> operational_semantics_step\<^sup>=\<^sup>= \<C>\<^sub>1 \<C>\<^sub>2\<close>
 
-abbreviation operational_semantics_step_relpowp :: "('\<tau>::linordered_field) config \<Rightarrow> nat \<Rightarrow> '\<tau> config \<Rightarrow> bool" ("_ \<hookrightarrow>\<^bsup>_\<^esup> _" 70) where
-  "\<C>\<^sub>1 \<hookrightarrow>\<^bsup>n\<^esup> \<C>\<^sub>2 \<equiv> (operational_semantics_step ^^ n) \<C>\<^sub>1 \<C>\<^sub>2"
+abbreviation operational_semantics_step_relpowp
+  ::\<open>('\<tau>::linordered_field) config \<Rightarrow> nat \<Rightarrow> '\<tau> config \<Rightarrow> bool\<close>         ("_ \<hookrightarrow>\<^bsup>_\<^esup> _" 70)
+where
+  \<open>\<C>\<^sub>1 \<hookrightarrow>\<^bsup>n\<^esup> \<C>\<^sub>2 \<equiv> (operational_semantics_step ^^ n) \<C>\<^sub>1 \<C>\<^sub>2\<close>
 
-definition operational_semantics_elim_inv :: "('\<tau>::linordered_field) config \<Rightarrow> '\<tau> config \<Rightarrow> bool" ("_ \<hookrightarrow>\<^sub>e\<^sup>\<leftarrow> _" 70) where
-  "\<C>\<^sub>1 \<hookrightarrow>\<^sub>e\<^sup>\<leftarrow> \<C>\<^sub>2 \<equiv> \<C>\<^sub>2 \<hookrightarrow>\<^sub>e \<C>\<^sub>1"
+definition operational_semantics_elim_inv
+  ::\<open>('\<tau>::linordered_field) config \<Rightarrow> '\<tau> config \<Rightarrow> bool\<close>                ("_ \<hookrightarrow>\<^sub>e\<^sup>\<leftarrow> _" 70)
+where
+  \<open>\<C>\<^sub>1 \<hookrightarrow>\<^sub>e\<^sup>\<leftarrow> \<C>\<^sub>2 \<equiv> \<C>\<^sub>2 \<hookrightarrow>\<^sub>e \<C>\<^sub>1\<close>
 
 
 section\<open>Basic Lemmas\<close>
 
 lemma operational_semantics_trans_generalized:
-  assumes "\<C>\<^sub>1 \<hookrightarrow>\<^bsup>n\<^esup> \<C>\<^sub>2"
-  assumes "\<C>\<^sub>2 \<hookrightarrow>\<^bsup>m\<^esup> \<C>\<^sub>3"
-  shows "\<C>\<^sub>1 \<hookrightarrow>\<^bsup>n + m\<^esup> \<C>\<^sub>3"
-  by (metis (no_types, hide_lams) assms(1) assms(2) relcompp.relcompI relpowp_add)
+  assumes \<open>\<C>\<^sub>1 \<hookrightarrow>\<^bsup>n\<^esup> \<C>\<^sub>2\<close>
+  assumes \<open>\<C>\<^sub>2 \<hookrightarrow>\<^bsup>m\<^esup> \<C>\<^sub>3\<close>
+    shows \<open>\<C>\<^sub>1 \<hookrightarrow>\<^bsup>n + m\<^esup> \<C>\<^sub>3\<close>
+using relcompp.relcompI[of  \<open>operational_semantics_step ^^ n\<close> _ _ 
+                            \<open>operational_semantics_step ^^ m\<close>, OF assms]
+by (simp add: relpowp_add) 
 
-abbreviation Cnext_solve :: "('\<tau>::linordered_field) config \<Rightarrow> '\<tau> config set" ("\<C>\<^sub>n\<^sub>e\<^sub>x\<^sub>t _") where
-  "\<C>\<^sub>n\<^sub>e\<^sub>x\<^sub>t \<S> \<equiv> { \<S>'. \<S> \<hookrightarrow> \<S>' }"
+abbreviation Cnext_solve
+  ::\<open>('\<tau>::linordered_field) config \<Rightarrow> '\<tau> config set\<close> ("\<C>\<^sub>n\<^sub>e\<^sub>x\<^sub>t _")
+where
+  \<open>\<C>\<^sub>n\<^sub>e\<^sub>x\<^sub>t \<S> \<equiv> { \<S>'. \<S> \<hookrightarrow> \<S>' }\<close>
 
 lemma Cnext_solve_instant:
-  shows "(\<C>\<^sub>n\<^sub>e\<^sub>x\<^sub>t (\<Gamma>, n \<turnstile> [] \<triangleright> \<Phi>))
-          \<supseteq> { \<Gamma>, Suc n \<turnstile> \<Phi> \<triangleright> [] }"
-  by (simp add: operational_semantics_step.simps operational_semantics_intro.instant_i)
+  \<open>(\<C>\<^sub>n\<^sub>e\<^sub>x\<^sub>t (\<Gamma>, n \<turnstile> [] \<triangleright> \<Phi>)) \<supseteq> { \<Gamma>, Suc n \<turnstile> \<Phi> \<triangleright> [] }\<close>
+by (simp add: operational_semantics_step.simps operational_semantics_intro.instant_i)
 
 lemma Cnext_solve_sporadicon:
-  shows "(\<C>\<^sub>n\<^sub>e\<^sub>x\<^sub>t (\<Gamma>, n \<turnstile> ((K\<^sub>1 sporadic \<tau> on K\<^sub>2) # \<Psi>) \<triangleright> \<Phi>))
-          \<supseteq> { \<Gamma>, n \<turnstile> \<Psi> \<triangleright> ((K\<^sub>1 sporadic \<tau> on K\<^sub>2) # \<Phi>),
-              ((K\<^sub>1 \<Up> n) # (K\<^sub>2 \<Down> n @ \<tau>) # \<Gamma>), n \<turnstile> \<Psi> \<triangleright> \<Phi> }"
-  by (simp add: operational_semantics_step.simps operational_semantics_elim.sporadic_on_e1 operational_semantics_elim.sporadic_on_e2)
+  \<open>(\<C>\<^sub>n\<^sub>e\<^sub>x\<^sub>t (\<Gamma>, n \<turnstile> ((K\<^sub>1 sporadic \<tau> on K\<^sub>2) # \<Psi>) \<triangleright> \<Phi>))
+    \<supseteq> { \<Gamma>, n \<turnstile> \<Psi> \<triangleright> ((K\<^sub>1 sporadic \<tau> on K\<^sub>2) # \<Phi>), ((K\<^sub>1 \<Up> n) # (K\<^sub>2 \<Down> n @ \<tau>) # \<Gamma>), n \<turnstile> \<Psi> \<triangleright> \<Phi> }\<close>
+by (simp add: operational_semantics_step.simps operational_semantics_elim.sporadic_on_e1
+              operational_semantics_elim.sporadic_on_e2)
 
 lemma Cnext_solve_tagrel:
-  shows "(\<C>\<^sub>n\<^sub>e\<^sub>x\<^sub>t (\<Gamma>, n \<turnstile> ((time-relation \<lfloor>K\<^sub>1, K\<^sub>2\<rfloor> \<in> R) # \<Psi>) \<triangleright> \<Phi>))
-          \<supseteq> { ((\<lfloor>\<tau>\<^sub>v\<^sub>a\<^sub>r(K\<^sub>1, n), \<tau>\<^sub>v\<^sub>a\<^sub>r(K\<^sub>2, n)\<rfloor> \<in> R) # \<Gamma>), n \<turnstile> \<Psi> \<triangleright> ((time-relation \<lfloor>K\<^sub>1, K\<^sub>2\<rfloor> \<in> R) # \<Phi>) }"
-  by (simp add: operational_semantics_step.simps operational_semantics_elim.tagrel_e)
+  \<open>(\<C>\<^sub>n\<^sub>e\<^sub>x\<^sub>t (\<Gamma>, n \<turnstile> ((time-relation \<lfloor>K\<^sub>1, K\<^sub>2\<rfloor> \<in> R) # \<Psi>) \<triangleright> \<Phi>))
+    \<supseteq> { ((\<lfloor>\<tau>\<^sub>v\<^sub>a\<^sub>r(K\<^sub>1, n), \<tau>\<^sub>v\<^sub>a\<^sub>r(K\<^sub>2, n)\<rfloor> \<in> R) # \<Gamma>), n \<turnstile> \<Psi> \<triangleright> ((time-relation \<lfloor>K\<^sub>1, K\<^sub>2\<rfloor> \<in> R) # \<Phi>) }\<close>
+by (simp add: operational_semantics_step.simps operational_semantics_elim.tagrel_e)
 
 lemma Cnext_solve_implies:
-  shows "(\<C>\<^sub>n\<^sub>e\<^sub>x\<^sub>t (\<Gamma>, n \<turnstile> ((K\<^sub>1 implies K\<^sub>2) # \<Psi>) \<triangleright> \<Phi>))
-          \<supseteq> { ((K\<^sub>1 \<not>\<Up> n) # \<Gamma>), n \<turnstile> \<Psi> \<triangleright> ((K\<^sub>1 implies K\<^sub>2) # \<Phi>),
-              ((K\<^sub>1 \<Up> n) # (K\<^sub>2 \<Up> n) # \<Gamma>), n \<turnstile> \<Psi> \<triangleright> ((K\<^sub>1 implies K\<^sub>2) # \<Phi>)}"
-  by (simp add: operational_semantics_step.simps operational_semantics_elim.implies_e1 operational_semantics_elim.implies_e2)
+  \<open>(\<C>\<^sub>n\<^sub>e\<^sub>x\<^sub>t (\<Gamma>, n \<turnstile> ((K\<^sub>1 implies K\<^sub>2) # \<Psi>) \<triangleright> \<Phi>))
+    \<supseteq> { ((K\<^sub>1 \<not>\<Up> n) # \<Gamma>), n \<turnstile> \<Psi> \<triangleright> ((K\<^sub>1 implies K\<^sub>2) # \<Phi>),
+         ((K\<^sub>1 \<Up> n) # (K\<^sub>2 \<Up> n) # \<Gamma>), n \<turnstile> \<Psi> \<triangleright> ((K\<^sub>1 implies K\<^sub>2) # \<Phi>) }\<close>
+by (simp add: operational_semantics_step.simps operational_semantics_elim.implies_e1
+              operational_semantics_elim.implies_e2)
 
 lemma Cnext_solve_implies_not:
-  shows "(\<C>\<^sub>n\<^sub>e\<^sub>x\<^sub>t (\<Gamma>, n \<turnstile> ((K\<^sub>1 implies not K\<^sub>2) # \<Psi>) \<triangleright> \<Phi>))
-          \<supseteq> { ((K\<^sub>1 \<not>\<Up> n) # \<Gamma>), n \<turnstile> \<Psi> \<triangleright> ((K\<^sub>1 implies not K\<^sub>2) # \<Phi>),
-              ((K\<^sub>1 \<Up> n) # (K\<^sub>2 \<not>\<Up> n) # \<Gamma>), n \<turnstile> \<Psi> \<triangleright> ((K\<^sub>1 implies not K\<^sub>2) # \<Phi>)}"
-  by (simp add: operational_semantics_step.simps operational_semantics_elim.implies_not_e1 operational_semantics_elim.implies_not_e2)
+  \<open>(\<C>\<^sub>n\<^sub>e\<^sub>x\<^sub>t (\<Gamma>, n \<turnstile> ((K\<^sub>1 implies not K\<^sub>2) # \<Psi>) \<triangleright> \<Phi>))
+    \<supseteq> { ((K\<^sub>1 \<not>\<Up> n) # \<Gamma>), n \<turnstile> \<Psi> \<triangleright> ((K\<^sub>1 implies not K\<^sub>2) # \<Phi>),
+        ((K\<^sub>1 \<Up> n) # (K\<^sub>2 \<not>\<Up> n) # \<Gamma>), n \<turnstile> \<Psi> \<triangleright> ((K\<^sub>1 implies not K\<^sub>2) # \<Phi>) }\<close>
+by (simp add: operational_semantics_step.simps operational_semantics_elim.implies_not_e1
+              operational_semantics_elim.implies_not_e2)
 
 lemma Cnext_solve_timedelayed:
-  shows "(\<C>\<^sub>n\<^sub>e\<^sub>x\<^sub>t (\<Gamma>, n \<turnstile> ((K\<^sub>1 time-delayed by \<delta>\<tau> on K\<^sub>2 implies K\<^sub>3) # \<Psi>) \<triangleright> \<Phi>))
-          \<supseteq> { ((K\<^sub>1 \<not>\<Up> n) # \<Gamma>), n \<turnstile> \<Psi> \<triangleright> ((K\<^sub>1 time-delayed by \<delta>\<tau> on K\<^sub>2 implies K\<^sub>3) # \<Phi>),
-              ((K\<^sub>1 \<Up> n) # (K\<^sub>2 @ n \<oplus> \<delta>\<tau> \<Rightarrow> K\<^sub>3) # \<Gamma>), n \<turnstile> \<Psi> \<triangleright> ((K\<^sub>1 time-delayed by \<delta>\<tau> on K\<^sub>2 implies K\<^sub>3) # \<Phi>) }"
-  by (simp add: operational_semantics_step.simps operational_semantics_elim.timedelayed_e1 operational_semantics_elim.timedelayed_e2)
+  \<open>(\<C>\<^sub>n\<^sub>e\<^sub>x\<^sub>t (\<Gamma>, n \<turnstile> ((K\<^sub>1 time-delayed by \<delta>\<tau> on K\<^sub>2 implies K\<^sub>3) # \<Psi>) \<triangleright> \<Phi>))
+    \<supseteq> { ((K\<^sub>1 \<not>\<Up> n) # \<Gamma>), n \<turnstile> \<Psi> \<triangleright> ((K\<^sub>1 time-delayed by \<delta>\<tau> on K\<^sub>2 implies K\<^sub>3) # \<Phi>),
+        ((K\<^sub>1 \<Up> n) # (K\<^sub>2 @ n \<oplus> \<delta>\<tau> \<Rightarrow> K\<^sub>3) # \<Gamma>), n
+          \<turnstile> \<Psi> \<triangleright> ((K\<^sub>1 time-delayed by \<delta>\<tau> on K\<^sub>2 implies K\<^sub>3) # \<Phi>) }\<close>
+by (simp add: operational_semantics_step.simps operational_semantics_elim.timedelayed_e1
+              operational_semantics_elim.timedelayed_e2)
 
 lemma Cnext_solve_weakly_precedes:
-  shows "(\<C>\<^sub>n\<^sub>e\<^sub>x\<^sub>t (\<Gamma>, n \<turnstile> ((K\<^sub>1 weakly precedes K\<^sub>2) # \<Psi>) \<triangleright> \<Phi>))
-          \<supseteq> { ((\<lceil>#\<^sup>\<le> K\<^sub>2 n, #\<^sup>\<le> K\<^sub>1 n\<rceil> \<in> (\<lambda>(x,y). x\<le>y)) # \<Gamma>), n \<turnstile> \<Psi> \<triangleright> ((K\<^sub>1 weakly precedes K\<^sub>2) # \<Phi>) }"
-  by (simp add: operational_semantics_step.simps operational_semantics_elim.weakly_precedes_e)
+  \<open>(\<C>\<^sub>n\<^sub>e\<^sub>x\<^sub>t (\<Gamma>, n \<turnstile> ((K\<^sub>1 weakly precedes K\<^sub>2) # \<Psi>) \<triangleright> \<Phi>))
+    \<supseteq> { ((\<lceil>#\<^sup>\<le> K\<^sub>2 n, #\<^sup>\<le> K\<^sub>1 n\<rceil> \<in> (\<lambda>(x,y). x\<le>y)) # \<Gamma>), n \<turnstile> \<Psi> \<triangleright> ((K\<^sub>1 weakly precedes K\<^sub>2) # \<Phi>) }\<close>
+by (simp add: operational_semantics_step.simps operational_semantics_elim.weakly_precedes_e)
 
 lemma Cnext_solve_strictly_precedes:
-  shows "(\<C>\<^sub>n\<^sub>e\<^sub>x\<^sub>t (\<Gamma>, n \<turnstile> ((K\<^sub>1 strictly precedes K\<^sub>2) # \<Psi>) \<triangleright> \<Phi>))
-          \<supseteq> { ((\<lceil>#\<^sup>\<le> K\<^sub>2 n, #\<^sup>< K\<^sub>1 n\<rceil> \<in> (\<lambda>(x,y). x\<le>y)) # \<Gamma>), n \<turnstile> \<Psi> \<triangleright> ((K\<^sub>1 strictly precedes K\<^sub>2) # \<Phi>) }"
-  by (simp add: operational_semantics_step.simps operational_semantics_elim.strictly_precedes_e)
+  \<open>(\<C>\<^sub>n\<^sub>e\<^sub>x\<^sub>t (\<Gamma>, n \<turnstile> ((K\<^sub>1 strictly precedes K\<^sub>2) # \<Psi>) \<triangleright> \<Phi>))
+    \<supseteq> { ((\<lceil>#\<^sup>\<le> K\<^sub>2 n, #\<^sup>< K\<^sub>1 n\<rceil> \<in> (\<lambda>(x,y). x\<le>y)) # \<Gamma>), n \<turnstile> \<Psi> \<triangleright> ((K\<^sub>1 strictly precedes K\<^sub>2) # \<Phi>) }\<close>
+by (simp add: operational_semantics_step.simps operational_semantics_elim.strictly_precedes_e)
 
 lemma Cnext_solve_kills:
-  shows "(\<C>\<^sub>n\<^sub>e\<^sub>x\<^sub>t (\<Gamma>, n \<turnstile> ((K\<^sub>1 kills K\<^sub>2) # \<Psi>) \<triangleright> \<Phi>))
-          \<supseteq> { ((K\<^sub>1 \<not>\<Up> n) # \<Gamma>), n \<turnstile> \<Psi> \<triangleright> ((K\<^sub>1 kills K\<^sub>2) # \<Phi>),
-              ((K\<^sub>1 \<Up> n) # (K\<^sub>2 \<not>\<Up> \<ge> n) # \<Gamma>), n \<turnstile> \<Psi> \<triangleright> ((K\<^sub>1 kills K\<^sub>2) # \<Phi>)}"
-  by (simp add: operational_semantics_step.simps operational_semantics_elim.kills_e1 operational_semantics_elim.kills_e2)
+  \<open>(\<C>\<^sub>n\<^sub>e\<^sub>x\<^sub>t (\<Gamma>, n \<turnstile> ((K\<^sub>1 kills K\<^sub>2) # \<Psi>) \<triangleright> \<Phi>))
+    \<supseteq> { ((K\<^sub>1 \<not>\<Up> n) # \<Gamma>), n \<turnstile> \<Psi> \<triangleright> ((K\<^sub>1 kills K\<^sub>2) # \<Phi>),
+        ((K\<^sub>1 \<Up> n) # (K\<^sub>2 \<not>\<Up> \<ge> n) # \<Gamma>), n \<turnstile> \<Psi> \<triangleright> ((K\<^sub>1 kills K\<^sub>2) # \<Phi>) }\<close>
+by (simp add: operational_semantics_step.simps operational_semantics_elim.kills_e1
+              operational_semantics_elim.kills_e2)
 
 lemma empty_spec_reductions:
-  shows "([], 0 \<turnstile> [] \<triangleright> []) \<hookrightarrow>\<^bsup>k\<^esup> ([], k \<turnstile> [] \<triangleright> [])"
-  proof (induct k)
-    case 0
-    then show ?case by simp
-  next
-    case (Suc k)
-    then show ?case
-      using instant_i operational_semantics_step.simps by fastforce 
-  qed
+  \<open>([], 0 \<turnstile> [] \<triangleright> []) \<hookrightarrow>\<^bsup>k\<^esup> ([], k \<turnstile> [] \<triangleright> [])\<close>
+proof (induct k)
+  case 0 thus ?case by simp
+next
+  case Suc thus ?case
+    using instant_i operational_semantics_step.simps by fastforce 
+qed
 
 end
