src/Denotational.thy
@@ -52,162 +52,172 @@ fun TESL_interpretation :: \<open>('\<tau>::linordered_field) TESL_formula \<Rig
 
 lemma TESL_interpretation_homo:
   \<open>\<lbrakk> \<phi> \<rbrakk>\<^sub>T\<^sub>E\<^sub>S\<^sub>L \<inter> \<lbrakk>\<lbrakk> \<Phi> \<rbrakk>\<rbrakk>\<^sub>T\<^sub>E\<^sub>S\<^sub>L = \<lbrakk>\<lbrakk> \<phi> # \<Phi> \<rbrakk>\<rbrakk>\<^sub>T\<^sub>E\<^sub>S\<^sub>L\<close>
-  by auto
+by auto
 
 subsection \<open>Image interpretation lemma\<close>
 
 theorem TESL_interpretation_image:
   \<open>\<lbrakk>\<lbrakk> \<Phi> \<rbrakk>\<rbrakk>\<^sub>T\<^sub>E\<^sub>S\<^sub>L = \<Inter> ((\<lambda>\<phi>. \<lbrakk> \<phi> \<rbrakk>\<^sub>T\<^sub>E\<^sub>S\<^sub>L) ` set \<Phi>)\<close>
-  proof (induct \<Phi>)
-    case Nil
-    then show ?case by simp
-  next
-    case (Cons a \<Phi>)
-    then show ?case by auto
-  qed
+proof (induct \<Phi>)
+  case Nil
+  then show ?case by simp
+next
+  case (Cons a \<Phi>)
+  then show ?case by auto
+qed
 
 subsection \<open>Expansion law\<close>
 text \<open>Similar to the expansion laws of lattices\<close>
 
 theorem TESL_interp_homo_append:
-  shows \<open>\<lbrakk>\<lbrakk> \<Phi>\<^sub>1 @ \<Phi>\<^sub>2 \<rbrakk>\<rbrakk>\<^sub>T\<^sub>E\<^sub>S\<^sub>L = \<lbrakk>\<lbrakk> \<Phi>\<^sub>1 \<rbrakk>\<rbrakk>\<^sub>T\<^sub>E\<^sub>S\<^sub>L \<inter> \<lbrakk>\<lbrakk> \<Phi>\<^sub>2 \<rbrakk>\<rbrakk>\<^sub>T\<^sub>E\<^sub>S\<^sub>L\<close>
-  proof (induct \<Phi>\<^sub>1)
-    case Nil
-    then show ?case by simp
-  next
-    case (Cons a \<Phi>\<^sub>1)
-    then show ?case by auto
-  qed
+  \<open>\<lbrakk>\<lbrakk> \<Phi>\<^sub>1 @ \<Phi>\<^sub>2 \<rbrakk>\<rbrakk>\<^sub>T\<^sub>E\<^sub>S\<^sub>L = \<lbrakk>\<lbrakk> \<Phi>\<^sub>1 \<rbrakk>\<rbrakk>\<^sub>T\<^sub>E\<^sub>S\<^sub>L \<inter> \<lbrakk>\<lbrakk> \<Phi>\<^sub>2 \<rbrakk>\<rbrakk>\<^sub>T\<^sub>E\<^sub>S\<^sub>L\<close>
+proof (induct \<Phi>\<^sub>1)
+  case Nil
+  then show ?case by simp
+next
+  case (Cons a \<Phi>\<^sub>1)
+  then show ?case by auto
+qed
 
 
 section \<open>Equational laws for TESL formulae denotationally interpreted\<close>
 
 lemma TESL_interp_assoc:
-  shows \<open>\<lbrakk>\<lbrakk> (\<Phi>\<^sub>1 @ \<Phi>\<^sub>2) @ \<Phi>\<^sub>3 \<rbrakk>\<rbrakk>\<^sub>T\<^sub>E\<^sub>S\<^sub>L = \<lbrakk>\<lbrakk> \<Phi>\<^sub>1 @ (\<Phi>\<^sub>2 @ \<Phi>\<^sub>3) \<rbrakk>\<rbrakk>\<^sub>T\<^sub>E\<^sub>S\<^sub>L\<close>
+  \<open>\<lbrakk>\<lbrakk> (\<Phi>\<^sub>1 @ \<Phi>\<^sub>2) @ \<Phi>\<^sub>3 \<rbrakk>\<rbrakk>\<^sub>T\<^sub>E\<^sub>S\<^sub>L = \<lbrakk>\<lbrakk> \<Phi>\<^sub>1 @ (\<Phi>\<^sub>2 @ \<Phi>\<^sub>3) \<rbrakk>\<rbrakk>\<^sub>T\<^sub>E\<^sub>S\<^sub>L\<close>
   by auto
 
 lemma TESL_interp_commute:
   shows \<open>\<lbrakk>\<lbrakk> \<Phi>\<^sub>1 @ \<Phi>\<^sub>2 \<rbrakk>\<rbrakk>\<^sub>T\<^sub>E\<^sub>S\<^sub>L = \<lbrakk>\<lbrakk> \<Phi>\<^sub>2 @ \<Phi>\<^sub>1 \<rbrakk>\<rbrakk>\<^sub>T\<^sub>E\<^sub>S\<^sub>L\<close>
-  by (simp add: TESL_interp_homo_append inf_sup_aci(1))
+by (simp add: TESL_interp_homo_append inf_sup_aci(1))
 
 lemma TESL_interp_left_commute:
-  shows \<open>\<lbrakk>\<lbrakk> \<Phi>\<^sub>1 @ (\<Phi>\<^sub>2 @ \<Phi>\<^sub>3) \<rbrakk>\<rbrakk>\<^sub>T\<^sub>E\<^sub>S\<^sub>L = \<lbrakk>\<lbrakk> \<Phi>\<^sub>2 @ (\<Phi>\<^sub>1 @ \<Phi>\<^sub>3) \<rbrakk>\<rbrakk>\<^sub>T\<^sub>E\<^sub>S\<^sub>L\<close>
-  unfolding TESL_interp_homo_append by auto
+  \<open>\<lbrakk>\<lbrakk> \<Phi>\<^sub>1 @ (\<Phi>\<^sub>2 @ \<Phi>\<^sub>3) \<rbrakk>\<rbrakk>\<^sub>T\<^sub>E\<^sub>S\<^sub>L = \<lbrakk>\<lbrakk> \<Phi>\<^sub>2 @ (\<Phi>\<^sub>1 @ \<Phi>\<^sub>3) \<rbrakk>\<rbrakk>\<^sub>T\<^sub>E\<^sub>S\<^sub>L\<close>
+unfolding TESL_interp_homo_append by auto
 
 lemma TESL_interp_idem:
-  shows \<open>\<lbrakk>\<lbrakk> \<Phi> @ \<Phi> \<rbrakk>\<rbrakk>\<^sub>T\<^sub>E\<^sub>S\<^sub>L = \<lbrakk>\<lbrakk> \<Phi> \<rbrakk>\<rbrakk>\<^sub>T\<^sub>E\<^sub>S\<^sub>L\<close>
-  using TESL_interp_homo_append by auto
+  \<open>\<lbrakk>\<lbrakk> \<Phi> @ \<Phi> \<rbrakk>\<rbrakk>\<^sub>T\<^sub>E\<^sub>S\<^sub>L = \<lbrakk>\<lbrakk> \<Phi> \<rbrakk>\<rbrakk>\<^sub>T\<^sub>E\<^sub>S\<^sub>L\<close>
+using TESL_interp_homo_append by auto
 
 lemma TESL_interp_left_idem:
-  shows \<open>\<lbrakk>\<lbrakk> \<Phi>\<^sub>1 @ (\<Phi>\<^sub>1 @ \<Phi>\<^sub>2) \<rbrakk>\<rbrakk>\<^sub>T\<^sub>E\<^sub>S\<^sub>L = \<lbrakk>\<lbrakk> \<Phi>\<^sub>1 @ \<Phi>\<^sub>2 \<rbrakk>\<rbrakk>\<^sub>T\<^sub>E\<^sub>S\<^sub>L\<close>
-  using TESL_interp_homo_append by auto
+  \<open>\<lbrakk>\<lbrakk> \<Phi>\<^sub>1 @ (\<Phi>\<^sub>1 @ \<Phi>\<^sub>2) \<rbrakk>\<rbrakk>\<^sub>T\<^sub>E\<^sub>S\<^sub>L = \<lbrakk>\<lbrakk> \<Phi>\<^sub>1 @ \<Phi>\<^sub>2 \<rbrakk>\<rbrakk>\<^sub>T\<^sub>E\<^sub>S\<^sub>L\<close>
+using TESL_interp_homo_append by auto
 
 lemma TESL_interp_right_idem:
-  shows \<open>\<lbrakk>\<lbrakk> (\<Phi>\<^sub>1 @ \<Phi>\<^sub>2) @ \<Phi>\<^sub>2 \<rbrakk>\<rbrakk>\<^sub>T\<^sub>E\<^sub>S\<^sub>L = \<lbrakk>\<lbrakk> \<Phi>\<^sub>1 @ \<Phi>\<^sub>2 \<rbrakk>\<rbrakk>\<^sub>T\<^sub>E\<^sub>S\<^sub>L\<close>
-  unfolding TESL_interp_homo_append by auto
+  \<open>\<lbrakk>\<lbrakk> (\<Phi>\<^sub>1 @ \<Phi>\<^sub>2) @ \<Phi>\<^sub>2 \<rbrakk>\<rbrakk>\<^sub>T\<^sub>E\<^sub>S\<^sub>L = \<lbrakk>\<lbrakk> \<Phi>\<^sub>1 @ \<Phi>\<^sub>2 \<rbrakk>\<rbrakk>\<^sub>T\<^sub>E\<^sub>S\<^sub>L\<close>
+unfolding TESL_interp_homo_append by auto
 
 lemmas TESL_interp_aci = TESL_interp_commute TESL_interp_assoc TESL_interp_left_commute TESL_interp_left_idem
 
 (* Identity element *)
 lemma TESL_interp_neutral1:
-  shows \<open>\<lbrakk>\<lbrakk> [] @ \<Phi> \<rbrakk>\<rbrakk>\<^sub>T\<^sub>E\<^sub>S\<^sub>L = \<lbrakk>\<lbrakk> \<Phi> \<rbrakk>\<rbrakk>\<^sub>T\<^sub>E\<^sub>S\<^sub>L\<close>
-  by simp
+  \<open>\<lbrakk>\<lbrakk> [] @ \<Phi> \<rbrakk>\<rbrakk>\<^sub>T\<^sub>E\<^sub>S\<^sub>L = \<lbrakk>\<lbrakk> \<Phi> \<rbrakk>\<rbrakk>\<^sub>T\<^sub>E\<^sub>S\<^sub>L\<close>
+by simp
 
 lemma TESL_interp_neutral2:
-  shows \<open>\<lbrakk>\<lbrakk> \<Phi> @ [] \<rbrakk>\<rbrakk>\<^sub>T\<^sub>E\<^sub>S\<^sub>L = \<lbrakk>\<lbrakk> \<Phi> \<rbrakk>\<rbrakk>\<^sub>T\<^sub>E\<^sub>S\<^sub>L\<close>
-  by simp
+  \<open>\<lbrakk>\<lbrakk> \<Phi> @ [] \<rbrakk>\<rbrakk>\<^sub>T\<^sub>E\<^sub>S\<^sub>L = \<lbrakk>\<lbrakk> \<Phi> \<rbrakk>\<rbrakk>\<^sub>T\<^sub>E\<^sub>S\<^sub>L\<close>
+by simp
 
 section \<open>Decreasing interpretation of TESL formulae\<close>
 
 lemma TESL_sem_decreases_head:
   \<open>\<lbrakk>\<lbrakk> \<Phi> \<rbrakk>\<rbrakk>\<^sub>T\<^sub>E\<^sub>S\<^sub>L \<supseteq> \<lbrakk>\<lbrakk> \<phi> # \<Phi> \<rbrakk>\<rbrakk>\<^sub>T\<^sub>E\<^sub>S\<^sub>L\<close>
-  by simp
+by simp
 
 lemma TESL_sem_decreases_tail:
   \<open>\<lbrakk>\<lbrakk> \<Phi> \<rbrakk>\<rbrakk>\<^sub>T\<^sub>E\<^sub>S\<^sub>L \<supseteq> \<lbrakk>\<lbrakk> \<Phi> @ [\<phi>] \<rbrakk>\<rbrakk>\<^sub>T\<^sub>E\<^sub>S\<^sub>L\<close>
-  by (simp add: TESL_interp_homo_append)
+by (simp add: TESL_interp_homo_append)
+
+lemma \<open>\<phi>#\<Phi> = [\<phi>]@\<Phi>\<close> by simp
 
 lemma TESL_interp_formula_stuttering:
-  assumes bel: \<open>\<phi> \<in> set \<Phi>\<close>
-  shows \<open>\<lbrakk>\<lbrakk> \<phi> # \<Phi> \<rbrakk>\<rbrakk>\<^sub>T\<^sub>E\<^sub>S\<^sub>L = \<lbrakk>\<lbrakk> \<Phi> \<rbrakk>\<rbrakk>\<^sub>T\<^sub>E\<^sub>S\<^sub>L\<close>
-  by (metis Int_subset_iff TESL_interp_homo_append TESL_interpretation.simps(2) bel in_set_conv_decomp_first subset_antisym subset_refl)
+  assumes \<open>\<phi> \<in> set \<Phi>\<close>
+    shows \<open>\<lbrakk>\<lbrakk> \<phi> # \<Phi> \<rbrakk>\<rbrakk>\<^sub>T\<^sub>E\<^sub>S\<^sub>L = \<lbrakk>\<lbrakk> \<Phi> \<rbrakk>\<rbrakk>\<^sub>T\<^sub>E\<^sub>S\<^sub>L\<close>
+proof -
+  have \<open>\<phi> # \<Phi> = [\<phi>] @ \<Phi>\<close> by simp
+  hence \<open>\<lbrakk>\<lbrakk> \<phi> # \<Phi> \<rbrakk>\<rbrakk>\<^sub>T\<^sub>E\<^sub>S\<^sub>L = \<lbrakk>\<lbrakk> [\<phi>] \<rbrakk>\<rbrakk>\<^sub>T\<^sub>E\<^sub>S\<^sub>L \<inter> \<lbrakk>\<lbrakk> \<Phi> \<rbrakk>\<rbrakk>\<^sub>T\<^sub>E\<^sub>S\<^sub>L\<close> using TESL_interp_homo_append by simp
+  thus ?thesis using assms TESL_interpretation_image by fastforce
+qed
 
 lemma TESL_interp_decreases:
-  shows \<open>\<lbrakk>\<lbrakk> \<Phi> \<rbrakk>\<rbrakk>\<^sub>T\<^sub>E\<^sub>S\<^sub>L \<supseteq> \<lbrakk>\<lbrakk> \<phi> # \<Phi> \<rbrakk>\<rbrakk>\<^sub>T\<^sub>E\<^sub>S\<^sub>L\<close>
-  by (rule TESL_sem_decreases_head)
+  \<open>\<lbrakk>\<lbrakk> \<Phi> \<rbrakk>\<rbrakk>\<^sub>T\<^sub>E\<^sub>S\<^sub>L \<supseteq> \<lbrakk>\<lbrakk> \<phi> # \<Phi> \<rbrakk>\<rbrakk>\<^sub>T\<^sub>E\<^sub>S\<^sub>L\<close>
+by (rule TESL_sem_decreases_head)
 
 lemma TESL_interp_remdups_absorb:
-  shows \<open>\<lbrakk>\<lbrakk> \<Phi> \<rbrakk>\<rbrakk>\<^sub>T\<^sub>E\<^sub>S\<^sub>L = \<lbrakk>\<lbrakk> remdups \<Phi> \<rbrakk>\<rbrakk>\<^sub>T\<^sub>E\<^sub>S\<^sub>L\<close>
-  proof (induct \<Phi>)
-    case Nil
-    then show ?case by simp
-  next
-    case (Cons a \<Phi>)
-    then show ?case
-      using TESL_interp_formula_stuttering by auto
-  qed
+  \<open>\<lbrakk>\<lbrakk> \<Phi> \<rbrakk>\<rbrakk>\<^sub>T\<^sub>E\<^sub>S\<^sub>L = \<lbrakk>\<lbrakk> remdups \<Phi> \<rbrakk>\<rbrakk>\<^sub>T\<^sub>E\<^sub>S\<^sub>L\<close>
+proof (induct \<Phi>)
+  case Nil
+  then show ?case by simp
+next
+  case (Cons a \<Phi>)
+  then show ?case
+    using TESL_interp_formula_stuttering by auto
+qed
 
 lemma TESL_interp_set_lifting:
   assumes \<open>set \<Phi> = set \<Phi>'\<close>
-  shows \<open>\<lbrakk>\<lbrakk> \<Phi> \<rbrakk>\<rbrakk>\<^sub>T\<^sub>E\<^sub>S\<^sub>L = \<lbrakk>\<lbrakk> \<Phi>' \<rbrakk>\<rbrakk>\<^sub>T\<^sub>E\<^sub>S\<^sub>L\<close>
-  proof -     
-    have \<open>set (remdups \<Phi>) = set (remdups \<Phi>')\<close>
-      by (simp add: assms)
-    moreover have fxpnt\<Phi>: \<open>\<Inter> ((\<lambda>\<phi>. \<lbrakk> \<phi> \<rbrakk>\<^sub>T\<^sub>E\<^sub>S\<^sub>L) ` set \<Phi>) = \<lbrakk>\<lbrakk> \<Phi> \<rbrakk>\<rbrakk>\<^sub>T\<^sub>E\<^sub>S\<^sub>L\<close>
-      by (simp add: TESL_interpretation_image)
-    moreover have fxpnt\<Phi>': \<open>\<Inter> ((\<lambda>\<phi>. \<lbrakk> \<phi> \<rbrakk>\<^sub>T\<^sub>E\<^sub>S\<^sub>L) ` set \<Phi>') = \<lbrakk>\<lbrakk> \<Phi>' \<rbrakk>\<rbrakk>\<^sub>T\<^sub>E\<^sub>S\<^sub>L\<close>
-      by (simp add: TESL_interpretation_image)
-    moreover have \<open>\<Inter> ((\<lambda>\<phi>. \<lbrakk> \<phi> \<rbrakk>\<^sub>T\<^sub>E\<^sub>S\<^sub>L) ` set \<Phi>) = \<Inter> ((\<lambda>\<phi>. \<lbrakk> \<phi> \<rbrakk>\<^sub>T\<^sub>E\<^sub>S\<^sub>L) ` set \<Phi>')\<close>
-      by (simp add: assms)
-    ultimately show ?thesis using TESL_interp_remdups_absorb by auto
-  qed
+    shows \<open>\<lbrakk>\<lbrakk> \<Phi> \<rbrakk>\<rbrakk>\<^sub>T\<^sub>E\<^sub>S\<^sub>L = \<lbrakk>\<lbrakk> \<Phi>' \<rbrakk>\<rbrakk>\<^sub>T\<^sub>E\<^sub>S\<^sub>L\<close>
+proof -     
+  have \<open>set (remdups \<Phi>) = set (remdups \<Phi>')\<close>
+    by (simp add: assms)
+  moreover have fxpnt\<Phi>: \<open>\<Inter> ((\<lambda>\<phi>. \<lbrakk> \<phi> \<rbrakk>\<^sub>T\<^sub>E\<^sub>S\<^sub>L) ` set \<Phi>) = \<lbrakk>\<lbrakk> \<Phi> \<rbrakk>\<rbrakk>\<^sub>T\<^sub>E\<^sub>S\<^sub>L\<close>
+    by (simp add: TESL_interpretation_image)
+  moreover have fxpnt\<Phi>': \<open>\<Inter> ((\<lambda>\<phi>. \<lbrakk> \<phi> \<rbrakk>\<^sub>T\<^sub>E\<^sub>S\<^sub>L) ` set \<Phi>') = \<lbrakk>\<lbrakk> \<Phi>' \<rbrakk>\<rbrakk>\<^sub>T\<^sub>E\<^sub>S\<^sub>L\<close>
+    by (simp add: TESL_interpretation_image)
+  moreover have \<open>\<Inter> ((\<lambda>\<phi>. \<lbrakk> \<phi> \<rbrakk>\<^sub>T\<^sub>E\<^sub>S\<^sub>L) ` set \<Phi>) = \<Inter> ((\<lambda>\<phi>. \<lbrakk> \<phi> \<rbrakk>\<^sub>T\<^sub>E\<^sub>S\<^sub>L) ` set \<Phi>')\<close>
+    by (simp add: assms)
+  ultimately show ?thesis using TESL_interp_remdups_absorb by auto
+qed
 
 theorem TESL_interp_decreases_setinc:
-  assumes incl: \<open>set \<Phi> \<subseteq> set \<Phi>'\<close>
-  shows \<open>\<lbrakk>\<lbrakk> \<Phi> \<rbrakk>\<rbrakk>\<^sub>T\<^sub>E\<^sub>S\<^sub>L \<supseteq> \<lbrakk>\<lbrakk> \<Phi>' \<rbrakk>\<rbrakk>\<^sub>T\<^sub>E\<^sub>S\<^sub>L\<close>
-  proof -
-    obtain \<Phi>\<^sub>r where decompose: \<open>set (\<Phi> @ \<Phi>\<^sub>r) = set \<Phi>'\<close> using incl by auto
-    have \<open>set (\<Phi> @ \<Phi>\<^sub>r) = set \<Phi>'\<close> using incl decompose by blast
-    moreover have \<open>(set \<Phi>) \<union> (set \<Phi>\<^sub>r) = set \<Phi>'\<close> using incl decompose by auto
-    moreover have \<open>\<lbrakk>\<lbrakk> \<Phi>' \<rbrakk>\<rbrakk>\<^sub>T\<^sub>E\<^sub>S\<^sub>L = \<lbrakk>\<lbrakk> \<Phi> @ \<Phi>\<^sub>r \<rbrakk>\<rbrakk>\<^sub>T\<^sub>E\<^sub>S\<^sub>L\<close> using TESL_interp_set_lifting decompose by blast
-    moreover have \<open>\<lbrakk>\<lbrakk> \<Phi> @ \<Phi>\<^sub>r \<rbrakk>\<rbrakk>\<^sub>T\<^sub>E\<^sub>S\<^sub>L = \<lbrakk>\<lbrakk> \<Phi> \<rbrakk>\<rbrakk>\<^sub>T\<^sub>E\<^sub>S\<^sub>L \<inter> \<lbrakk>\<lbrakk> \<Phi>\<^sub>r \<rbrakk>\<rbrakk>\<^sub>T\<^sub>E\<^sub>S\<^sub>L\<close> by (simp add: TESL_interp_homo_append)
-    moreover have \<open>\<lbrakk>\<lbrakk> \<Phi> \<rbrakk>\<rbrakk>\<^sub>T\<^sub>E\<^sub>S\<^sub>L \<supseteq> \<lbrakk>\<lbrakk> \<Phi> \<rbrakk>\<rbrakk>\<^sub>T\<^sub>E\<^sub>S\<^sub>L \<inter> \<lbrakk>\<lbrakk> \<Phi>\<^sub>r \<rbrakk>\<rbrakk>\<^sub>T\<^sub>E\<^sub>S\<^sub>L\<close> by simp
-    ultimately show ?thesis by simp
-  qed
+  assumes \<open>set \<Phi> \<subseteq> set \<Phi>'\<close>
+    shows \<open>\<lbrakk>\<lbrakk> \<Phi> \<rbrakk>\<rbrakk>\<^sub>T\<^sub>E\<^sub>S\<^sub>L \<supseteq> \<lbrakk>\<lbrakk> \<Phi>' \<rbrakk>\<rbrakk>\<^sub>T\<^sub>E\<^sub>S\<^sub>L\<close>
+proof -
+  obtain \<Phi>\<^sub>r where decompose: \<open>set (\<Phi> @ \<Phi>\<^sub>r) = set \<Phi>'\<close> using assms by auto
+  have \<open>set (\<Phi> @ \<Phi>\<^sub>r) = set \<Phi>'\<close> using assms decompose by blast
+  moreover have \<open>(set \<Phi>) \<union> (set \<Phi>\<^sub>r) = set \<Phi>'\<close> using assms decompose by auto
+  moreover have \<open>\<lbrakk>\<lbrakk> \<Phi>' \<rbrakk>\<rbrakk>\<^sub>T\<^sub>E\<^sub>S\<^sub>L = \<lbrakk>\<lbrakk> \<Phi> @ \<Phi>\<^sub>r \<rbrakk>\<rbrakk>\<^sub>T\<^sub>E\<^sub>S\<^sub>L\<close> using TESL_interp_set_lifting decompose by blast
+  moreover have \<open>\<lbrakk>\<lbrakk> \<Phi> @ \<Phi>\<^sub>r \<rbrakk>\<rbrakk>\<^sub>T\<^sub>E\<^sub>S\<^sub>L = \<lbrakk>\<lbrakk> \<Phi> \<rbrakk>\<rbrakk>\<^sub>T\<^sub>E\<^sub>S\<^sub>L \<inter> \<lbrakk>\<lbrakk> \<Phi>\<^sub>r \<rbrakk>\<rbrakk>\<^sub>T\<^sub>E\<^sub>S\<^sub>L\<close> by (simp add: TESL_interp_homo_append)
+  moreover have \<open>\<lbrakk>\<lbrakk> \<Phi> \<rbrakk>\<rbrakk>\<^sub>T\<^sub>E\<^sub>S\<^sub>L \<supseteq> \<lbrakk>\<lbrakk> \<Phi> \<rbrakk>\<rbrakk>\<^sub>T\<^sub>E\<^sub>S\<^sub>L \<inter> \<lbrakk>\<lbrakk> \<Phi>\<^sub>r \<rbrakk>\<rbrakk>\<^sub>T\<^sub>E\<^sub>S\<^sub>L\<close> by simp
+  ultimately show ?thesis by simp
+qed
 
 lemma TESL_interp_decreases_add_head:
-  assumes incl: \<open>set \<Phi> \<subseteq> set \<Phi>'\<close>
-  shows \<open>\<lbrakk>\<lbrakk> \<phi> # \<Phi> \<rbrakk>\<rbrakk>\<^sub>T\<^sub>E\<^sub>S\<^sub>L \<supseteq> \<lbrakk>\<lbrakk> \<phi> # \<Phi>' \<rbrakk>\<rbrakk>\<^sub>T\<^sub>E\<^sub>S\<^sub>L\<close>
-  using TESL_interp_decreases_setinc incl by auto
+  assumes \<open>set \<Phi> \<subseteq> set \<Phi>'\<close>
+    shows \<open>\<lbrakk>\<lbrakk> \<phi> # \<Phi> \<rbrakk>\<rbrakk>\<^sub>T\<^sub>E\<^sub>S\<^sub>L \<supseteq> \<lbrakk>\<lbrakk> \<phi> # \<Phi>' \<rbrakk>\<rbrakk>\<^sub>T\<^sub>E\<^sub>S\<^sub>L\<close>
+using assms TESL_interp_decreases_setinc by auto
 
 lemma TESL_interp_decreases_add_tail:
-  assumes incl: \<open>set \<Phi> \<subseteq> set \<Phi>'\<close>
-  shows \<open>\<lbrakk>\<lbrakk> \<Phi> @ [\<phi>] \<rbrakk>\<rbrakk>\<^sub>T\<^sub>E\<^sub>S\<^sub>L \<supseteq> \<lbrakk>\<lbrakk> \<Phi>' @ [\<phi>] \<rbrakk>\<rbrakk>\<^sub>T\<^sub>E\<^sub>S\<^sub>L\<close>
-  by (metis TESL_interp_commute TESL_interp_decreases_add_head append_Cons append_Nil incl)
+  assumes \<open>set \<Phi> \<subseteq> set \<Phi>'\<close>
+    shows \<open>\<lbrakk>\<lbrakk> \<Phi> @ [\<phi>] \<rbrakk>\<rbrakk>\<^sub>T\<^sub>E\<^sub>S\<^sub>L \<supseteq> \<lbrakk>\<lbrakk> \<Phi>' @ [\<phi>] \<rbrakk>\<rbrakk>\<^sub>T\<^sub>E\<^sub>S\<^sub>L\<close>
+using TESL_interp_decreases_setinc[OF assms] 
+  by (simp add: TESL_interpretation_image dual_order.trans)
 
 lemma TESL_interp_absorb1:
-  assumes incl: \<open>set \<Phi>\<^sub>1 \<subseteq> set \<Phi>\<^sub>2\<close>
-  shows \<open>\<lbrakk>\<lbrakk> \<Phi>\<^sub>1 @ \<Phi>\<^sub>2 \<rbrakk>\<rbrakk>\<^sub>T\<^sub>E\<^sub>S\<^sub>L = \<lbrakk>\<lbrakk> \<Phi>\<^sub>2 \<rbrakk>\<rbrakk>\<^sub>T\<^sub>E\<^sub>S\<^sub>L\<close>
-  by (simp add: Int_absorb1 TESL_interp_decreases_setinc TESL_interp_homo_append incl)
+  assumes \<open>set \<Phi>\<^sub>1 \<subseteq> set \<Phi>\<^sub>2\<close>
+    shows \<open>\<lbrakk>\<lbrakk> \<Phi>\<^sub>1 @ \<Phi>\<^sub>2 \<rbrakk>\<rbrakk>\<^sub>T\<^sub>E\<^sub>S\<^sub>L = \<lbrakk>\<lbrakk> \<Phi>\<^sub>2 \<rbrakk>\<rbrakk>\<^sub>T\<^sub>E\<^sub>S\<^sub>L\<close>
+by (simp add: Int_absorb1 TESL_interp_decreases_setinc TESL_interp_homo_append assms)
 
 lemma TESL_interp_absorb2:
-  assumes incl: \<open>set \<Phi>\<^sub>2 \<subseteq> set \<Phi>\<^sub>1\<close>
-  shows \<open>\<lbrakk>\<lbrakk> \<Phi>\<^sub>1 @ \<Phi>\<^sub>2 \<rbrakk>\<rbrakk>\<^sub>T\<^sub>E\<^sub>S\<^sub>L = \<lbrakk>\<lbrakk> \<Phi>\<^sub>1 \<rbrakk>\<rbrakk>\<^sub>T\<^sub>E\<^sub>S\<^sub>L\<close>
-  using TESL_interp_absorb1 TESL_interp_commute incl by blast
+  assumes \<open>set \<Phi>\<^sub>2 \<subseteq> set \<Phi>\<^sub>1\<close>
+    shows \<open>\<lbrakk>\<lbrakk> \<Phi>\<^sub>1 @ \<Phi>\<^sub>2 \<rbrakk>\<rbrakk>\<^sub>T\<^sub>E\<^sub>S\<^sub>L = \<lbrakk>\<lbrakk> \<Phi>\<^sub>1 \<rbrakk>\<rbrakk>\<^sub>T\<^sub>E\<^sub>S\<^sub>L\<close>
+using TESL_interp_absorb1 TESL_interp_commute assms by blast
 
 section \<open>Some special cases\<close>
 
 lemma NoSporadic_stable [simp]:
-  shows \<open>\<lbrakk>\<lbrakk> \<Phi> \<rbrakk>\<rbrakk>\<^sub>T\<^sub>E\<^sub>S\<^sub>L \<subseteq> \<lbrakk>\<lbrakk> NoSporadic \<Phi> \<rbrakk>\<rbrakk>\<^sub>T\<^sub>E\<^sub>S\<^sub>L\<close>
-  by (meson filter_is_subset TESL_interp_decreases_setinc)
+  \<open>\<lbrakk>\<lbrakk> \<Phi> \<rbrakk>\<rbrakk>\<^sub>T\<^sub>E\<^sub>S\<^sub>L \<subseteq> \<lbrakk>\<lbrakk> NoSporadic \<Phi> \<rbrakk>\<rbrakk>\<^sub>T\<^sub>E\<^sub>S\<^sub>L\<close>
+proof -
+  from filter_is_subset have \<open>set (NoSporadic \<Phi>) \<subseteq> set \<Phi>\<close> .
+  from TESL_interp_decreases_setinc[OF this] show ?thesis .
+qed
 
 lemma NoSporadic_idem [simp]:
-  shows \<open>\<lbrakk>\<lbrakk> \<Phi> \<rbrakk>\<rbrakk>\<^sub>T\<^sub>E\<^sub>S\<^sub>L \<inter> \<lbrakk>\<lbrakk> NoSporadic \<Phi> \<rbrakk>\<rbrakk>\<^sub>T\<^sub>E\<^sub>S\<^sub>L = \<lbrakk>\<lbrakk> \<Phi> \<rbrakk>\<rbrakk>\<^sub>T\<^sub>E\<^sub>S\<^sub>L\<close>
-  by (meson Int_absorb2 filter_is_subset TESL_interp_decreases_setinc)
+  \<open>\<lbrakk>\<lbrakk> \<Phi> \<rbrakk>\<rbrakk>\<^sub>T\<^sub>E\<^sub>S\<^sub>L \<inter> \<lbrakk>\<lbrakk> NoSporadic \<Phi> \<rbrakk>\<rbrakk>\<^sub>T\<^sub>E\<^sub>S\<^sub>L = \<lbrakk>\<lbrakk> \<Phi> \<rbrakk>\<rbrakk>\<^sub>T\<^sub>E\<^sub>S\<^sub>L\<close>
+using NoSporadic_stable by blast
 
 lemma NoSporadic_setinc:
-  shows \<open>set (NoSporadic \<Phi>) \<subseteq> set \<Phi>\<close>
-  by auto
+  \<open>set (NoSporadic \<Phi>) \<subseteq> set \<Phi>\<close>
+by (rule filter_is_subset)
 
 (*<*)
 no_notation dummyT0    ("t\<^sub>0")
