src/SymbolicPrimitive.thy
@@ -3,20 +3,20 @@ theory SymbolicPrimitive
 
 begin
 datatype cnt_expr =
-    TickCountLess \<open>clock\<close> \<open>instant_index\<close>  ("#\<^sup><")
-  | TickCountLeq \<open>clock\<close> \<open>instant_index\<close> ("#\<^sup>\<le>")
+  TickCountLess \<open>clock\<close> \<open>instant_index\<close> ("#\<^sup><")
+| TickCountLeq \<open>clock\<close> \<open>instant_index\<close>  ("#\<^sup>\<le>")
 
 subsection\<open> Symbolic Primitives for Runs \<close>
 datatype '\<tau> constr =
-    Timestamp     \<open>clock\<close>   \<open>instant_index\<close> \<open>'\<tau> tag_const\<close>         ("_ \<Down> _ @ _")
-  | TimeDelay     \<open>clock\<close>   \<open>instant_index\<close> \<open>'\<tau> tag_const\<close> \<open>clock\<close> ("_ @ _ \<oplus> _ \<Rightarrow> _")
-  | Ticks         \<open>clock\<close>   \<open>instant_index\<close>                        ("_ \<Up> _")
-  | NotTicks      \<open>clock\<close>   \<open>instant_index\<close>                        ("_ \<not>\<Up> _")
-  | NotTicksUntil \<open>clock\<close>   \<open>instant_index\<close>                        ("_ \<not>\<Up> < _")
-  | NotTicksFrom  \<open>clock\<close>   \<open>instant_index\<close>                        ("_ \<not>\<Up> \<ge> _")
-  | TagArith      \<open>tag_var\<close> \<open>tag_var\<close> \<open>('\<tau> tag_const \<times> '\<tau> tag_const) \<Rightarrow> bool\<close> ("\<lfloor>_, _\<rfloor> \<in> _")
-  | TickCntArith  \<open>cnt_expr\<close> \<open>cnt_expr\<close> \<open>(nat \<times> nat) \<Rightarrow> bool\<close>               ("\<lceil>_, _\<rceil> \<in> _")
-  | TickCntLeq    \<open>cnt_expr\<close> \<open>cnt_expr\<close>                           ("_ \<preceq> _")
+  Timestamp     \<open>clock\<close>   \<open>instant_index\<close> \<open>'\<tau> tag_const\<close>         ("_ \<Down> _ @ _")
+| TimeDelay     \<open>clock\<close>   \<open>instant_index\<close> \<open>'\<tau> tag_const\<close> \<open>clock\<close> ("_ @ _ \<oplus> _ \<Rightarrow> _")
+| Ticks         \<open>clock\<close>   \<open>instant_index\<close>                        ("_ \<Up> _")
+| NotTicks      \<open>clock\<close>   \<open>instant_index\<close>                        ("_ \<not>\<Up> _")
+| NotTicksUntil \<open>clock\<close>   \<open>instant_index\<close>                        ("_ \<not>\<Up> < _")
+| NotTicksFrom  \<open>clock\<close>   \<open>instant_index\<close>                        ("_ \<not>\<Up> \<ge> _")
+| TagArith      \<open>tag_var\<close> \<open>tag_var\<close> \<open>('\<tau> tag_const \<times> '\<tau> tag_const) \<Rightarrow> bool\<close> ("\<lfloor>_, _\<rfloor> \<in> _")
+| TickCntArith  \<open>cnt_expr\<close> \<open>cnt_expr\<close> \<open>(nat \<times> nat) \<Rightarrow> bool\<close>      ("\<lceil>_, _\<rceil> \<in> _")
+| TickCntLeq    \<open>cnt_expr\<close> \<open>cnt_expr\<close>                            ("_ \<preceq> _")
 
 type_synonym '\<tau> system = \<open>'\<tau> constr list\<close>
 
@@ -33,31 +33,37 @@ section \<open>Semantics of Primitive Constraints \<close>
 
 fun counter_expr_eval :: \<open>('\<tau>::linordered_field) run \<Rightarrow> cnt_expr \<Rightarrow> nat\<close> ("\<lbrakk> _ \<turnstile> _ \<rbrakk>\<^sub>c\<^sub>n\<^sub>t\<^sub>e\<^sub>x\<^sub>p\<^sub>r")
 where
-    \<open>\<lbrakk> \<rho> \<turnstile> #\<^sup>< clk indx \<rbrakk>\<^sub>c\<^sub>n\<^sub>t\<^sub>e\<^sub>x\<^sub>p\<^sub>r = run_tick_count_strictly \<rho> clk indx\<close>
-  | \<open>\<lbrakk> \<rho> \<turnstile> #\<^sup>\<le> clk indx \<rbrakk>\<^sub>c\<^sub>n\<^sub>t\<^sub>e\<^sub>x\<^sub>p\<^sub>r = run_tick_count \<rho> clk indx\<close>
+  \<open>\<lbrakk> \<rho> \<turnstile> #\<^sup>< clk indx \<rbrakk>\<^sub>c\<^sub>n\<^sub>t\<^sub>e\<^sub>x\<^sub>p\<^sub>r = run_tick_count_strictly \<rho> clk indx\<close>
+| \<open>\<lbrakk> \<rho> \<turnstile> #\<^sup>\<le> clk indx \<rbrakk>\<^sub>c\<^sub>n\<^sub>t\<^sub>e\<^sub>x\<^sub>p\<^sub>r = run_tick_count \<rho> clk indx\<close>
 
 
-fun symbolic_run_interpretation_primitive :: \<open>('\<tau>::linordered_field) constr \<Rightarrow> '\<tau> run set\<close> ("\<lbrakk> _ \<rbrakk>\<^sub>p\<^sub>r\<^sub>i\<^sub>m")
+fun symbolic_run_interpretation_primitive
+  ::\<open>('\<tau>::linordered_field) constr \<Rightarrow> '\<tau> run set\<close> ("\<lbrakk> _ \<rbrakk>\<^sub>p\<^sub>r\<^sub>i\<^sub>m")
 where
-    \<open>\<lbrakk> K \<Up> n  \<rbrakk>\<^sub>p\<^sub>r\<^sub>i\<^sub>m     = { \<rho>. hamlet ((Rep_run \<rho>) n K) }\<close>
-  | \<open>\<lbrakk> K @ n\<^sub>0 \<oplus> \<delta>t \<Rightarrow> K' \<rbrakk>\<^sub>p\<^sub>r\<^sub>i\<^sub>m = { \<rho>. \<forall>n \<ge> n\<^sub>0. first_time \<rho> K n (time ((Rep_run \<rho>) n\<^sub>0 K) + \<delta>t) \<longrightarrow> hamlet ((Rep_run \<rho>) n K')}\<close>
-  | \<open>\<lbrakk> K \<not>\<Up> n \<rbrakk>\<^sub>p\<^sub>r\<^sub>i\<^sub>m     = { \<rho>. \<not>hamlet ((Rep_run \<rho>) n K) }\<close>
-  | \<open>\<lbrakk> K \<not>\<Up> < n \<rbrakk>\<^sub>p\<^sub>r\<^sub>i\<^sub>m   = { \<rho>. \<forall>i < n. \<not> hamlet ((Rep_run \<rho>) i K)}\<close>
-  | \<open>\<lbrakk> K \<not>\<Up> \<ge> n \<rbrakk>\<^sub>p\<^sub>r\<^sub>i\<^sub>m   = { \<rho>. \<forall>i \<ge> n. \<not> hamlet ((Rep_run \<rho>) i K) }\<close>
-  | \<open>\<lbrakk> K \<Down> n @ \<tau> \<rbrakk>\<^sub>p\<^sub>r\<^sub>i\<^sub>m = { \<rho>. time ((Rep_run \<rho>) n K) = \<tau> }\<close>
-  | \<open>\<lbrakk> \<lfloor>\<tau>\<^sub>v\<^sub>a\<^sub>r(K\<^sub>1, n\<^sub>1), \<tau>\<^sub>v\<^sub>a\<^sub>r(K\<^sub>2, n\<^sub>2)\<rfloor> \<in> R \<rbrakk>\<^sub>p\<^sub>r\<^sub>i\<^sub>m = { \<rho>. R (time ((Rep_run \<rho>) n\<^sub>1 K\<^sub>1), time ((Rep_run \<rho>) n\<^sub>2 K\<^sub>2)) }\<close>
-  | \<open>\<lbrakk> \<lceil>e\<^sub>1, e\<^sub>2\<rceil> \<in> R \<rbrakk>\<^sub>p\<^sub>r\<^sub>i\<^sub>m = { \<rho>. R (\<lbrakk> \<rho> \<turnstile> e\<^sub>1 \<rbrakk>\<^sub>c\<^sub>n\<^sub>t\<^sub>e\<^sub>x\<^sub>p\<^sub>r, \<lbrakk> \<rho> \<turnstile> e\<^sub>2 \<rbrakk>\<^sub>c\<^sub>n\<^sub>t\<^sub>e\<^sub>x\<^sub>p\<^sub>r) }\<close>
-  | \<open>\<lbrakk> cnt_e\<^sub>1 \<preceq> cnt_e\<^sub>2 \<rbrakk>\<^sub>p\<^sub>r\<^sub>i\<^sub>m = { \<rho>. \<lbrakk> \<rho> \<turnstile> cnt_e\<^sub>1 \<rbrakk>\<^sub>c\<^sub>n\<^sub>t\<^sub>e\<^sub>x\<^sub>p\<^sub>r \<le> \<lbrakk> \<rho> \<turnstile> cnt_e\<^sub>2 \<rbrakk>\<^sub>c\<^sub>n\<^sub>t\<^sub>e\<^sub>x\<^sub>p\<^sub>r }\<close>
+  \<open>\<lbrakk> K \<Up> n  \<rbrakk>\<^sub>p\<^sub>r\<^sub>i\<^sub>m     = {\<rho>. hamlet ((Rep_run \<rho>) n K) }\<close>
+| \<open>\<lbrakk> K @ n\<^sub>0 \<oplus> \<delta>t \<Rightarrow> K' \<rbrakk>\<^sub>p\<^sub>r\<^sub>i\<^sub>m = {\<rho>. \<forall>n \<ge> n\<^sub>0. first_time \<rho> K n (time ((Rep_run \<rho>) n\<^sub>0 K) + \<delta>t)
+                                            \<longrightarrow> hamlet ((Rep_run \<rho>) n K')}\<close>
+| \<open>\<lbrakk> K \<not>\<Up> n \<rbrakk>\<^sub>p\<^sub>r\<^sub>i\<^sub>m     = {\<rho>. \<not>hamlet ((Rep_run \<rho>) n K) }\<close>
+| \<open>\<lbrakk> K \<not>\<Up> < n \<rbrakk>\<^sub>p\<^sub>r\<^sub>i\<^sub>m   = {\<rho>. \<forall>i < n. \<not> hamlet ((Rep_run \<rho>) i K)}\<close>
+| \<open>\<lbrakk> K \<not>\<Up> \<ge> n \<rbrakk>\<^sub>p\<^sub>r\<^sub>i\<^sub>m   = {\<rho>. \<forall>i \<ge> n. \<not> hamlet ((Rep_run \<rho>) i K) }\<close>
+| \<open>\<lbrakk> K \<Down> n @ \<tau> \<rbrakk>\<^sub>p\<^sub>r\<^sub>i\<^sub>m = {\<rho>. time ((Rep_run \<rho>) n K) = \<tau> }\<close>
+| \<open>\<lbrakk> \<lfloor>\<tau>\<^sub>v\<^sub>a\<^sub>r(K\<^sub>1, n\<^sub>1), \<tau>\<^sub>v\<^sub>a\<^sub>r(K\<^sub>2, n\<^sub>2)\<rfloor> \<in> R \<rbrakk>\<^sub>p\<^sub>r\<^sub>i\<^sub>m =
+    { \<rho>. R (time ((Rep_run \<rho>) n\<^sub>1 K\<^sub>1), time ((Rep_run \<rho>) n\<^sub>2 K\<^sub>2)) }\<close>
+| \<open>\<lbrakk> \<lceil>e\<^sub>1, e\<^sub>2\<rceil> \<in> R \<rbrakk>\<^sub>p\<^sub>r\<^sub>i\<^sub>m = { \<rho>. R (\<lbrakk> \<rho> \<turnstile> e\<^sub>1 \<rbrakk>\<^sub>c\<^sub>n\<^sub>t\<^sub>e\<^sub>x\<^sub>p\<^sub>r, \<lbrakk> \<rho> \<turnstile> e\<^sub>2 \<rbrakk>\<^sub>c\<^sub>n\<^sub>t\<^sub>e\<^sub>x\<^sub>p\<^sub>r) }\<close>
+| \<open>\<lbrakk> cnt_e\<^sub>1 \<preceq> cnt_e\<^sub>2 \<rbrakk>\<^sub>p\<^sub>r\<^sub>i\<^sub>m = { \<rho>. \<lbrakk> \<rho> \<turnstile> cnt_e\<^sub>1 \<rbrakk>\<^sub>c\<^sub>n\<^sub>t\<^sub>e\<^sub>x\<^sub>p\<^sub>r \<le> \<lbrakk> \<rho> \<turnstile> cnt_e\<^sub>2 \<rbrakk>\<^sub>c\<^sub>n\<^sub>t\<^sub>e\<^sub>x\<^sub>p\<^sub>r }\<close>
 
-fun symbolic_run_interpretation :: \<open>('\<tau>::linordered_field) constr list \<Rightarrow> ('\<tau>::linordered_field) run set\<close> ("\<lbrakk>\<lbrakk> _ \<rbrakk>\<rbrakk>\<^sub>p\<^sub>r\<^sub>i\<^sub>m") where
-    \<open>\<lbrakk>\<lbrakk> [] \<rbrakk>\<rbrakk>\<^sub>p\<^sub>r\<^sub>i\<^sub>m = { _. True }\<close>
-  | \<open>\<lbrakk>\<lbrakk> \<gamma> # \<Gamma> \<rbrakk>\<rbrakk>\<^sub>p\<^sub>r\<^sub>i\<^sub>m = \<lbrakk> \<gamma> \<rbrakk>\<^sub>p\<^sub>r\<^sub>i\<^sub>m \<inter> \<lbrakk>\<lbrakk> \<Gamma> \<rbrakk>\<rbrakk>\<^sub>p\<^sub>r\<^sub>i\<^sub>m\<close>
+fun symbolic_run_interpretation
+  ::\<open>('\<tau>::linordered_field) constr list \<Rightarrow> ('\<tau>::linordered_field) run set\<close> ("\<lbrakk>\<lbrakk> _ \<rbrakk>\<rbrakk>\<^sub>p\<^sub>r\<^sub>i\<^sub>m")
+where
+  \<open>\<lbrakk>\<lbrakk> [] \<rbrakk>\<rbrakk>\<^sub>p\<^sub>r\<^sub>i\<^sub>m = { _. True }\<close>
+| \<open>\<lbrakk>\<lbrakk> \<gamma> # \<Gamma> \<rbrakk>\<rbrakk>\<^sub>p\<^sub>r\<^sub>i\<^sub>m = \<lbrakk> \<gamma> \<rbrakk>\<^sub>p\<^sub>r\<^sub>i\<^sub>m \<inter> \<lbrakk>\<lbrakk> \<Gamma> \<rbrakk>\<rbrakk>\<^sub>p\<^sub>r\<^sub>i\<^sub>m\<close>
 
 lemma symbolic_run_interp_cons_morph:
   \<open>\<lbrakk> \<gamma> \<rbrakk>\<^sub>p\<^sub>r\<^sub>i\<^sub>m \<inter> \<lbrakk>\<lbrakk> \<Gamma> \<rbrakk>\<rbrakk>\<^sub>p\<^sub>r\<^sub>i\<^sub>m = \<lbrakk>\<lbrakk> \<gamma> # \<Gamma> \<rbrakk>\<rbrakk>\<^sub>p\<^sub>r\<^sub>i\<^sub>m\<close>
-  by auto
+by auto
 
-definition consistent_context :: \<open>('\<tau>::linordered_field) constr list \<Rightarrow> bool\<close> where 
+definition consistent_context :: \<open>('\<tau>::linordered_field) constr list \<Rightarrow> bool\<close>
+where 
   \<open>consistent_context \<Gamma> \<equiv> \<exists>\<rho>. \<rho> \<in> \<lbrakk>\<lbrakk> \<Gamma> \<rbrakk>\<rbrakk>\<^sub>p\<^sub>r\<^sub>i\<^sub>m\<close>
 
 subsection \<open>Defining a method for witness construction\<close> (**)
@@ -68,8 +74,10 @@ abbreviation initial_run :: \<open>('\<tau>::linordered_field) run\<close> ("\<r
 
 \<comment> \<open>To ensure monotonicity, time tag is set at a specific instant and forever after (stuttering)\<close>
 fun time_update
-  :: \<open>nat \<Rightarrow> clock \<Rightarrow> ('\<tau>::linordered_field) tag_const \<Rightarrow> (nat \<Rightarrow> clock \<Rightarrow> (bool \<times> '\<tau> tag_const)) \<Rightarrow> (nat \<Rightarrow> clock \<Rightarrow> (bool \<times> '\<tau> tag_const))\<close> where
-    \<open>time_update n K \<tau> \<rho> = (\<lambda>n' K'. if K = K' \<and> n \<le> n' then (hamlet (\<rho> n K), \<tau>) else \<rho> n' K')\<close>
+  :: \<open>nat \<Rightarrow> clock \<Rightarrow> ('\<tau>::linordered_field) tag_const \<Rightarrow> (nat \<Rightarrow> clock \<Rightarrow> (bool \<times> '\<tau> tag_const))
+      \<Rightarrow> (nat \<Rightarrow> clock \<Rightarrow> (bool \<times> '\<tau> tag_const))\<close>
+where
+  \<open>time_update n K \<tau> \<rho> = (\<lambda>n' K'. if K = K' \<and> n \<le> n' then (hamlet (\<rho> n K), \<tau>) else \<rho> n' K')\<close>
 
 
 section \<open>Rules and properties of consistence\<close> (**)
@@ -82,7 +90,8 @@ unfolding consistent_context_def
 by auto
 
 \<comment> \<open>This is very restrictive\<close>
-inductive context_independency :: \<open>('\<tau>::linordered_field) constr \<Rightarrow> '\<tau> constr list \<Rightarrow> bool\<close> ("_ \<bowtie> _") where
+inductive context_independency::\<open>('\<tau>::linordered_field) constr \<Rightarrow> '\<tau> constr list \<Rightarrow> bool\<close> ("_ \<bowtie> _")
+where
   NotTicks_independency:
   \<open>(K \<Up> n) \<notin> set \<Gamma> \<Longrightarrow> (K \<not>\<Up> n) \<bowtie> \<Gamma>\<close>
 | Ticks_independency:
@@ -90,149 +99,154 @@ inductive context_independency :: \<open>('\<tau>::linordered_field) constr \<Ri
 | Timestamp_independency:
   \<open>(\<nexists>\<tau>'. \<tau>' = \<tau> \<and> (K \<Down> n @ \<tau>) \<in> set \<Gamma>) \<Longrightarrow> (K \<Down> n @ \<tau>) \<bowtie> \<Gamma>\<close>
 
-
+\<^cancel>\<open>
 lemma context_consistency_preservationE:
   assumes consist: \<open>consistent_context \<Gamma>\<close>
   and     indepen: \<open>\<gamma> \<bowtie> \<Gamma>\<close>
   shows   \<open>consistent_context (\<gamma> # \<Gamma>)\<close>
   oops
-
+\<close>
 
 section\<open>Major Theorems\<close>
 subsection \<open>Fixpoint lemma\<close>
 
 theorem symrun_interp_fixpoint:
   \<open>\<Inter> ((\<lambda>\<gamma>. \<lbrakk> \<gamma> \<rbrakk>\<^sub>p\<^sub>r\<^sub>i\<^sub>m) ` set \<Gamma>) = \<lbrakk>\<lbrakk> \<Gamma> \<rbrakk>\<rbrakk>\<^sub>p\<^sub>r\<^sub>i\<^sub>m\<close>
-  proof (induct \<Gamma>)
-    case Nil
-    then show ?case by simp
-  next
-    case (Cons a \<Gamma>)
-    then show ?case by auto
-  qed
+proof (induct \<Gamma>)
+  case Nil thus ?case by simp
+next
+  case Cons thus ?case by auto
+qed
 
 subsection \<open>Expansion law\<close>
 text \<open>Similar to the expansion laws of lattices\<close>
 
 theorem symrun_interp_expansion:
-  shows \<open>\<lbrakk>\<lbrakk> \<Gamma>\<^sub>1 @ \<Gamma>\<^sub>2 \<rbrakk>\<rbrakk>\<^sub>p\<^sub>r\<^sub>i\<^sub>m = \<lbrakk>\<lbrakk> \<Gamma>\<^sub>1 \<rbrakk>\<rbrakk>\<^sub>p\<^sub>r\<^sub>i\<^sub>m \<inter> \<lbrakk>\<lbrakk> \<Gamma>\<^sub>2 \<rbrakk>\<rbrakk>\<^sub>p\<^sub>r\<^sub>i\<^sub>m\<close>
+  \<open>\<lbrakk>\<lbrakk> \<Gamma>\<^sub>1 @ \<Gamma>\<^sub>2 \<rbrakk>\<rbrakk>\<^sub>p\<^sub>r\<^sub>i\<^sub>m = \<lbrakk>\<lbrakk> \<Gamma>\<^sub>1 \<rbrakk>\<rbrakk>\<^sub>p\<^sub>r\<^sub>i\<^sub>m \<inter> \<lbrakk>\<lbrakk> \<Gamma>\<^sub>2 \<rbrakk>\<rbrakk>\<^sub>p\<^sub>r\<^sub>i\<^sub>m\<close>
 by (induction \<Gamma>\<^sub>1, auto)
 
 section \<open>Equational laws for TESL formulae denotationally interpreted\<close> 
 subsection \<open>General laws\<close>
 
 lemma symrun_interp_assoc:
-  shows \<open>\<lbrakk>\<lbrakk> (\<Gamma>\<^sub>1 @ \<Gamma>\<^sub>2) @ \<Gamma>\<^sub>3 \<rbrakk>\<rbrakk>\<^sub>p\<^sub>r\<^sub>i\<^sub>m = \<lbrakk>\<lbrakk> \<Gamma>\<^sub>1 @ (\<Gamma>\<^sub>2 @ \<Gamma>\<^sub>3) \<rbrakk>\<rbrakk>\<^sub>p\<^sub>r\<^sub>i\<^sub>m\<close>
-  by auto
+  \<open>\<lbrakk>\<lbrakk> (\<Gamma>\<^sub>1 @ \<Gamma>\<^sub>2) @ \<Gamma>\<^sub>3 \<rbrakk>\<rbrakk>\<^sub>p\<^sub>r\<^sub>i\<^sub>m = \<lbrakk>\<lbrakk> \<Gamma>\<^sub>1 @ (\<Gamma>\<^sub>2 @ \<Gamma>\<^sub>3) \<rbrakk>\<rbrakk>\<^sub>p\<^sub>r\<^sub>i\<^sub>m\<close>
+by auto
 
 lemma symrun_interp_commute:
-  shows \<open>\<lbrakk>\<lbrakk> \<Gamma>\<^sub>1 @ \<Gamma>\<^sub>2 \<rbrakk>\<rbrakk>\<^sub>p\<^sub>r\<^sub>i\<^sub>m = \<lbrakk>\<lbrakk> \<Gamma>\<^sub>2 @ \<Gamma>\<^sub>1 \<rbrakk>\<rbrakk>\<^sub>p\<^sub>r\<^sub>i\<^sub>m\<close>
-  by (simp add: symrun_interp_expansion inf_sup_aci(1))
+  \<open>\<lbrakk>\<lbrakk> \<Gamma>\<^sub>1 @ \<Gamma>\<^sub>2 \<rbrakk>\<rbrakk>\<^sub>p\<^sub>r\<^sub>i\<^sub>m = \<lbrakk>\<lbrakk> \<Gamma>\<^sub>2 @ \<Gamma>\<^sub>1 \<rbrakk>\<rbrakk>\<^sub>p\<^sub>r\<^sub>i\<^sub>m\<close>
+by (simp add: symrun_interp_expansion inf_sup_aci(1))
 
 lemma symrun_interp_left_commute:
-  shows \<open>\<lbrakk>\<lbrakk> \<Gamma>\<^sub>1 @ (\<Gamma>\<^sub>2 @ \<Gamma>\<^sub>3) \<rbrakk>\<rbrakk>\<^sub>p\<^sub>r\<^sub>i\<^sub>m = \<lbrakk>\<lbrakk> \<Gamma>\<^sub>2 @ (\<Gamma>\<^sub>1 @ \<Gamma>\<^sub>3) \<rbrakk>\<rbrakk>\<^sub>p\<^sub>r\<^sub>i\<^sub>m\<close>
-  unfolding symrun_interp_expansion by auto
+  \<open>\<lbrakk>\<lbrakk> \<Gamma>\<^sub>1 @ (\<Gamma>\<^sub>2 @ \<Gamma>\<^sub>3) \<rbrakk>\<rbrakk>\<^sub>p\<^sub>r\<^sub>i\<^sub>m = \<lbrakk>\<lbrakk> \<Gamma>\<^sub>2 @ (\<Gamma>\<^sub>1 @ \<Gamma>\<^sub>3) \<rbrakk>\<rbrakk>\<^sub>p\<^sub>r\<^sub>i\<^sub>m\<close>
+unfolding symrun_interp_expansion by auto
 
 lemma symrun_interp_idem:
-  shows \<open>\<lbrakk>\<lbrakk> \<Gamma> @ \<Gamma> \<rbrakk>\<rbrakk>\<^sub>p\<^sub>r\<^sub>i\<^sub>m = \<lbrakk>\<lbrakk> \<Gamma> \<rbrakk>\<rbrakk>\<^sub>p\<^sub>r\<^sub>i\<^sub>m\<close>
-  using symrun_interp_expansion by auto
+  \<open>\<lbrakk>\<lbrakk> \<Gamma> @ \<Gamma> \<rbrakk>\<rbrakk>\<^sub>p\<^sub>r\<^sub>i\<^sub>m = \<lbrakk>\<lbrakk> \<Gamma> \<rbrakk>\<rbrakk>\<^sub>p\<^sub>r\<^sub>i\<^sub>m\<close>
+using symrun_interp_expansion by auto
 
 lemma symrun_interp_left_idem:
-  shows \<open>\<lbrakk>\<lbrakk> \<Gamma>\<^sub>1 @ (\<Gamma>\<^sub>1 @ \<Gamma>\<^sub>2) \<rbrakk>\<rbrakk>\<^sub>p\<^sub>r\<^sub>i\<^sub>m = \<lbrakk>\<lbrakk> \<Gamma>\<^sub>1 @ \<Gamma>\<^sub>2 \<rbrakk>\<rbrakk>\<^sub>p\<^sub>r\<^sub>i\<^sub>m\<close>
-  using symrun_interp_expansion by auto
+  \<open>\<lbrakk>\<lbrakk> \<Gamma>\<^sub>1 @ (\<Gamma>\<^sub>1 @ \<Gamma>\<^sub>2) \<rbrakk>\<rbrakk>\<^sub>p\<^sub>r\<^sub>i\<^sub>m = \<lbrakk>\<lbrakk> \<Gamma>\<^sub>1 @ \<Gamma>\<^sub>2 \<rbrakk>\<rbrakk>\<^sub>p\<^sub>r\<^sub>i\<^sub>m\<close>
+using symrun_interp_expansion by auto
 
 lemma symrun_interp_right_idem:
-  shows \<open>\<lbrakk>\<lbrakk> (\<Gamma>\<^sub>1 @ \<Gamma>\<^sub>2) @ \<Gamma>\<^sub>2 \<rbrakk>\<rbrakk>\<^sub>p\<^sub>r\<^sub>i\<^sub>m = \<lbrakk>\<lbrakk> \<Gamma>\<^sub>1 @ \<Gamma>\<^sub>2 \<rbrakk>\<rbrakk>\<^sub>p\<^sub>r\<^sub>i\<^sub>m\<close>
-  unfolding symrun_interp_expansion by auto
+  \<open>\<lbrakk>\<lbrakk> (\<Gamma>\<^sub>1 @ \<Gamma>\<^sub>2) @ \<Gamma>\<^sub>2 \<rbrakk>\<rbrakk>\<^sub>p\<^sub>r\<^sub>i\<^sub>m = \<lbrakk>\<lbrakk> \<Gamma>\<^sub>1 @ \<Gamma>\<^sub>2 \<rbrakk>\<rbrakk>\<^sub>p\<^sub>r\<^sub>i\<^sub>m\<close>
+unfolding symrun_interp_expansion by auto
 
-lemmas symrun_interp_aci = symrun_interp_commute symrun_interp_assoc symrun_interp_left_commute symrun_interp_left_idem
+lemmas symrun_interp_aci =  symrun_interp_commute
+                            symrun_interp_assoc
+                            symrun_interp_left_commute
+                            symrun_interp_left_idem
 
 \<comment> \<open>Identity element\<close>
 lemma symrun_interp_neutral1:
-  shows \<open>\<lbrakk>\<lbrakk> [] @ \<Gamma> \<rbrakk>\<rbrakk>\<^sub>p\<^sub>r\<^sub>i\<^sub>m = \<lbrakk>\<lbrakk> \<Gamma> \<rbrakk>\<rbrakk>\<^sub>p\<^sub>r\<^sub>i\<^sub>m\<close>
-  by simp
+  \<open>\<lbrakk>\<lbrakk> [] @ \<Gamma> \<rbrakk>\<rbrakk>\<^sub>p\<^sub>r\<^sub>i\<^sub>m = \<lbrakk>\<lbrakk> \<Gamma> \<rbrakk>\<rbrakk>\<^sub>p\<^sub>r\<^sub>i\<^sub>m\<close>
+by simp
 
 lemma symrun_interp_neutral2:
-  shows \<open>\<lbrakk>\<lbrakk> \<Gamma> @ [] \<rbrakk>\<rbrakk>\<^sub>p\<^sub>r\<^sub>i\<^sub>m = \<lbrakk>\<lbrakk> \<Gamma> \<rbrakk>\<rbrakk>\<^sub>p\<^sub>r\<^sub>i\<^sub>m\<close>
-  by simp
+  \<open>\<lbrakk>\<lbrakk> \<Gamma> @ [] \<rbrakk>\<rbrakk>\<^sub>p\<^sub>r\<^sub>i\<^sub>m = \<lbrakk>\<lbrakk> \<Gamma> \<rbrakk>\<rbrakk>\<^sub>p\<^sub>r\<^sub>i\<^sub>m\<close>
+by simp
 
 subsection \<open>Decreasing interpretation of TESL formulae\<close>
 
 lemma TESL_sem_decreases_head:
   \<open>\<lbrakk>\<lbrakk> \<Gamma> \<rbrakk>\<rbrakk>\<^sub>p\<^sub>r\<^sub>i\<^sub>m \<supseteq> \<lbrakk>\<lbrakk> \<gamma> # \<Gamma> \<rbrakk>\<rbrakk>\<^sub>p\<^sub>r\<^sub>i\<^sub>m\<close>
-  by simp
+by simp
 
 lemma TESL_sem_decreases_tail:
   \<open>\<lbrakk>\<lbrakk> \<Gamma> \<rbrakk>\<rbrakk>\<^sub>p\<^sub>r\<^sub>i\<^sub>m \<supseteq> \<lbrakk>\<lbrakk> \<Gamma> @ [\<gamma>] \<rbrakk>\<rbrakk>\<^sub>p\<^sub>r\<^sub>i\<^sub>m\<close>
-  by (simp add: symrun_interp_expansion)
+by (simp add: symrun_interp_expansion)
 
 lemma symrun_interp_formula_stuttering:
-  assumes bel: \<open>\<gamma> \<in> set \<Gamma>\<close>
-  shows \<open>\<lbrakk>\<lbrakk> \<gamma> # \<Gamma> \<rbrakk>\<rbrakk>\<^sub>p\<^sub>r\<^sub>i\<^sub>m = \<lbrakk>\<lbrakk> \<Gamma> \<rbrakk>\<rbrakk>\<^sub>p\<^sub>r\<^sub>i\<^sub>m\<close>
-  by (metis Int_absorb1 Int_left_commute bel inf_le1 split_list symbolic_run_interpretation.simps(2) symrun_interp_expansion)
+  assumes \<open>\<gamma> \<in> set \<Gamma>\<close>
+    shows \<open>\<lbrakk>\<lbrakk> \<gamma> # \<Gamma> \<rbrakk>\<rbrakk>\<^sub>p\<^sub>r\<^sub>i\<^sub>m = \<lbrakk>\<lbrakk> \<Gamma> \<rbrakk>\<rbrakk>\<^sub>p\<^sub>r\<^sub>i\<^sub>m\<close>
+proof -
+  have \<open>\<gamma> # \<Gamma> = [\<gamma>] @ \<Gamma>\<close> by simp
+  hence \<open>\<lbrakk>\<lbrakk> \<gamma> # \<Gamma> \<rbrakk>\<rbrakk>\<^sub>p\<^sub>r\<^sub>i\<^sub>m = \<lbrakk>\<lbrakk> [\<gamma>] \<rbrakk>\<rbrakk>\<^sub>p\<^sub>r\<^sub>i\<^sub>m \<inter> \<lbrakk>\<lbrakk> \<Gamma> \<rbrakk>\<rbrakk>\<^sub>p\<^sub>r\<^sub>i\<^sub>m\<close> using symrun_interp_expansion by simp
+  thus ?thesis using assms symrun_interp_fixpoint by fastforce
+qed
 
 lemma symrun_interp_decreases:
-  shows \<open>\<lbrakk>\<lbrakk> \<Gamma> \<rbrakk>\<rbrakk>\<^sub>p\<^sub>r\<^sub>i\<^sub>m \<supseteq> \<lbrakk>\<lbrakk> \<gamma> # \<Gamma> \<rbrakk>\<rbrakk>\<^sub>p\<^sub>r\<^sub>i\<^sub>m\<close>
-  by (rule TESL_sem_decreases_head)
+  \<open>\<lbrakk>\<lbrakk> \<Gamma> \<rbrakk>\<rbrakk>\<^sub>p\<^sub>r\<^sub>i\<^sub>m \<supseteq> \<lbrakk>\<lbrakk> \<gamma> # \<Gamma> \<rbrakk>\<rbrakk>\<^sub>p\<^sub>r\<^sub>i\<^sub>m\<close>
+by (rule TESL_sem_decreases_head)
 
 lemma symrun_interp_remdups_absorb:
-  shows \<open>\<lbrakk>\<lbrakk> \<Gamma> \<rbrakk>\<rbrakk>\<^sub>p\<^sub>r\<^sub>i\<^sub>m = \<lbrakk>\<lbrakk> remdups \<Gamma> \<rbrakk>\<rbrakk>\<^sub>p\<^sub>r\<^sub>i\<^sub>m\<close>
-  proof (induct \<Gamma>)
-    case Nil
-    then show ?case by simp
-  next
-    case (Cons a \<Gamma>)
-    then show ?case
-      using symrun_interp_formula_stuttering by auto
-  qed
+  \<open>\<lbrakk>\<lbrakk> \<Gamma> \<rbrakk>\<rbrakk>\<^sub>p\<^sub>r\<^sub>i\<^sub>m = \<lbrakk>\<lbrakk> remdups \<Gamma> \<rbrakk>\<rbrakk>\<^sub>p\<^sub>r\<^sub>i\<^sub>m\<close>
+proof (induct \<Gamma>)
+  case Nil thus ?case by simp
+next
+  case Cons
+    thus ?case using symrun_interp_formula_stuttering by auto
+qed
 
 lemma symrun_interp_set_lifting:
   assumes \<open>set \<Gamma> = set \<Gamma>'\<close>
-  shows \<open>\<lbrakk>\<lbrakk> \<Gamma> \<rbrakk>\<rbrakk>\<^sub>p\<^sub>r\<^sub>i\<^sub>m = \<lbrakk>\<lbrakk> \<Gamma>' \<rbrakk>\<rbrakk>\<^sub>p\<^sub>r\<^sub>i\<^sub>m\<close>
-  proof -     
-    have \<open>set (remdups \<Gamma>) = set (remdups \<Gamma>')\<close>
-      by (simp add: assms)
-    moreover have fxpnt\<Gamma>: \<open>\<Inter> ((\<lambda>\<gamma>. \<lbrakk> \<gamma> \<rbrakk>\<^sub>p\<^sub>r\<^sub>i\<^sub>m) ` set \<Gamma>) = \<lbrakk>\<lbrakk> \<Gamma> \<rbrakk>\<rbrakk>\<^sub>p\<^sub>r\<^sub>i\<^sub>m\<close>
-      by (simp add: symrun_interp_fixpoint)
-    moreover have fxpnt\<Gamma>': \<open>\<Inter> ((\<lambda>\<gamma>. \<lbrakk> \<gamma> \<rbrakk>\<^sub>p\<^sub>r\<^sub>i\<^sub>m) ` set \<Gamma>') = \<lbrakk>\<lbrakk> \<Gamma>' \<rbrakk>\<rbrakk>\<^sub>p\<^sub>r\<^sub>i\<^sub>m\<close>
-      by (simp add: symrun_interp_fixpoint)
-    moreover have \<open>\<Inter> ((\<lambda>\<gamma>. \<lbrakk> \<gamma> \<rbrakk>\<^sub>p\<^sub>r\<^sub>i\<^sub>m) ` set \<Gamma>) = \<Inter> ((\<lambda>\<gamma>. \<lbrakk> \<gamma> \<rbrakk>\<^sub>p\<^sub>r\<^sub>i\<^sub>m) ` set \<Gamma>')\<close>
-      by (simp add: assms)
-    ultimately show ?thesis using symrun_interp_remdups_absorb by auto
-  qed
+    shows \<open>\<lbrakk>\<lbrakk> \<Gamma> \<rbrakk>\<rbrakk>\<^sub>p\<^sub>r\<^sub>i\<^sub>m = \<lbrakk>\<lbrakk> \<Gamma>' \<rbrakk>\<rbrakk>\<^sub>p\<^sub>r\<^sub>i\<^sub>m\<close>
+proof -     
+  have \<open>set (remdups \<Gamma>) = set (remdups \<Gamma>')\<close>
+    by (simp add: assms)
+  moreover have fxpnt\<Gamma>: \<open>\<Inter> ((\<lambda>\<gamma>. \<lbrakk> \<gamma> \<rbrakk>\<^sub>p\<^sub>r\<^sub>i\<^sub>m) ` set \<Gamma>) = \<lbrakk>\<lbrakk> \<Gamma> \<rbrakk>\<rbrakk>\<^sub>p\<^sub>r\<^sub>i\<^sub>m\<close>
+    by (simp add: symrun_interp_fixpoint)
+  moreover have fxpnt\<Gamma>': \<open>\<Inter> ((\<lambda>\<gamma>. \<lbrakk> \<gamma> \<rbrakk>\<^sub>p\<^sub>r\<^sub>i\<^sub>m) ` set \<Gamma>') = \<lbrakk>\<lbrakk> \<Gamma>' \<rbrakk>\<rbrakk>\<^sub>p\<^sub>r\<^sub>i\<^sub>m\<close>
+    by (simp add: symrun_interp_fixpoint)
+  moreover have \<open>\<Inter> ((\<lambda>\<gamma>. \<lbrakk> \<gamma> \<rbrakk>\<^sub>p\<^sub>r\<^sub>i\<^sub>m) ` set \<Gamma>) = \<Inter> ((\<lambda>\<gamma>. \<lbrakk> \<gamma> \<rbrakk>\<^sub>p\<^sub>r\<^sub>i\<^sub>m) ` set \<Gamma>')\<close>
+    by (simp add: assms)
+  ultimately show ?thesis using symrun_interp_remdups_absorb by auto
+qed
 
 theorem symrun_interp_decreases_setinc:
-  assumes incl: \<open>set \<Gamma> \<subseteq> set \<Gamma>'\<close>
-  shows \<open>\<lbrakk>\<lbrakk> \<Gamma> \<rbrakk>\<rbrakk>\<^sub>p\<^sub>r\<^sub>i\<^sub>m \<supseteq> \<lbrakk>\<lbrakk> \<Gamma>' \<rbrakk>\<rbrakk>\<^sub>p\<^sub>r\<^sub>i\<^sub>m\<close>
-  proof -
-    obtain \<Gamma>\<^sub>r where decompose: \<open>set (\<Gamma> @ \<Gamma>\<^sub>r) = set \<Gamma>'\<close> using incl by auto
-    have \<open>set (\<Gamma> @ \<Gamma>\<^sub>r) = set \<Gamma>'\<close> using incl decompose by blast
-    moreover have \<open>(set \<Gamma>) \<union> (set \<Gamma>\<^sub>r) = set \<Gamma>'\<close> using incl decompose by auto
-    moreover have \<open>\<lbrakk>\<lbrakk> \<Gamma>' \<rbrakk>\<rbrakk>\<^sub>p\<^sub>r\<^sub>i\<^sub>m = \<lbrakk>\<lbrakk> \<Gamma> @ \<Gamma>\<^sub>r \<rbrakk>\<rbrakk>\<^sub>p\<^sub>r\<^sub>i\<^sub>m\<close> using symrun_interp_set_lifting decompose by blast
-    moreover have \<open>\<lbrakk>\<lbrakk> \<Gamma> @ \<Gamma>\<^sub>r \<rbrakk>\<rbrakk>\<^sub>p\<^sub>r\<^sub>i\<^sub>m = \<lbrakk>\<lbrakk> \<Gamma> \<rbrakk>\<rbrakk>\<^sub>p\<^sub>r\<^sub>i\<^sub>m \<inter> \<lbrakk>\<lbrakk> \<Gamma>\<^sub>r \<rbrakk>\<rbrakk>\<^sub>p\<^sub>r\<^sub>i\<^sub>m\<close> by (simp add: symrun_interp_expansion)
-    moreover have \<open>\<lbrakk>\<lbrakk> \<Gamma> \<rbrakk>\<rbrakk>\<^sub>p\<^sub>r\<^sub>i\<^sub>m \<supseteq> \<lbrakk>\<lbrakk> \<Gamma> \<rbrakk>\<rbrakk>\<^sub>p\<^sub>r\<^sub>i\<^sub>m \<inter> \<lbrakk>\<lbrakk> \<Gamma>\<^sub>r \<rbrakk>\<rbrakk>\<^sub>p\<^sub>r\<^sub>i\<^sub>m\<close> by simp
-    ultimately show ?thesis by simp
-  qed
+  assumes \<open>set \<Gamma> \<subseteq> set \<Gamma>'\<close>
+    shows \<open>\<lbrakk>\<lbrakk> \<Gamma> \<rbrakk>\<rbrakk>\<^sub>p\<^sub>r\<^sub>i\<^sub>m \<supseteq> \<lbrakk>\<lbrakk> \<Gamma>' \<rbrakk>\<rbrakk>\<^sub>p\<^sub>r\<^sub>i\<^sub>m\<close>
+proof -
+  obtain \<Gamma>\<^sub>r where decompose: \<open>set (\<Gamma> @ \<Gamma>\<^sub>r) = set \<Gamma>'\<close> using assms by auto
+  have \<open>set (\<Gamma> @ \<Gamma>\<^sub>r) = set \<Gamma>'\<close> using assms decompose by blast
+  moreover have \<open>(set \<Gamma>) \<union> (set \<Gamma>\<^sub>r) = set \<Gamma>'\<close> using assms decompose by auto
+  moreover have \<open>\<lbrakk>\<lbrakk> \<Gamma>' \<rbrakk>\<rbrakk>\<^sub>p\<^sub>r\<^sub>i\<^sub>m = \<lbrakk>\<lbrakk> \<Gamma> @ \<Gamma>\<^sub>r \<rbrakk>\<rbrakk>\<^sub>p\<^sub>r\<^sub>i\<^sub>m\<close> using symrun_interp_set_lifting decompose by blast
+  moreover have \<open>\<lbrakk>\<lbrakk> \<Gamma> @ \<Gamma>\<^sub>r \<rbrakk>\<rbrakk>\<^sub>p\<^sub>r\<^sub>i\<^sub>m = \<lbrakk>\<lbrakk> \<Gamma> \<rbrakk>\<rbrakk>\<^sub>p\<^sub>r\<^sub>i\<^sub>m \<inter> \<lbrakk>\<lbrakk> \<Gamma>\<^sub>r \<rbrakk>\<rbrakk>\<^sub>p\<^sub>r\<^sub>i\<^sub>m\<close> by (simp add: symrun_interp_expansion)
+  moreover have \<open>\<lbrakk>\<lbrakk> \<Gamma> \<rbrakk>\<rbrakk>\<^sub>p\<^sub>r\<^sub>i\<^sub>m \<supseteq> \<lbrakk>\<lbrakk> \<Gamma> \<rbrakk>\<rbrakk>\<^sub>p\<^sub>r\<^sub>i\<^sub>m \<inter> \<lbrakk>\<lbrakk> \<Gamma>\<^sub>r \<rbrakk>\<rbrakk>\<^sub>p\<^sub>r\<^sub>i\<^sub>m\<close> by simp
+  ultimately show ?thesis by simp
+qed
 
 lemma symrun_interp_decreases_add_head:
-  assumes incl: \<open>set \<Gamma> \<subseteq> set \<Gamma>'\<close>
-  shows \<open>\<lbrakk>\<lbrakk> \<gamma> # \<Gamma> \<rbrakk>\<rbrakk>\<^sub>p\<^sub>r\<^sub>i\<^sub>m \<supseteq> \<lbrakk>\<lbrakk> \<gamma> # \<Gamma>' \<rbrakk>\<rbrakk>\<^sub>p\<^sub>r\<^sub>i\<^sub>m\<close>
-  using symrun_interp_decreases_setinc incl by auto
+  assumes \<open>set \<Gamma> \<subseteq> set \<Gamma>'\<close>
+    shows \<open>\<lbrakk>\<lbrakk> \<gamma> # \<Gamma> \<rbrakk>\<rbrakk>\<^sub>p\<^sub>r\<^sub>i\<^sub>m \<supseteq> \<lbrakk>\<lbrakk> \<gamma> # \<Gamma>' \<rbrakk>\<rbrakk>\<^sub>p\<^sub>r\<^sub>i\<^sub>m\<close>
+using symrun_interp_decreases_setinc assms by auto
 
 lemma symrun_interp_decreases_add_tail:
-  assumes incl: \<open>set \<Gamma> \<subseteq> set \<Gamma>'\<close>
-  shows \<open>\<lbrakk>\<lbrakk> \<Gamma> @ [\<gamma>] \<rbrakk>\<rbrakk>\<^sub>p\<^sub>r\<^sub>i\<^sub>m \<supseteq> \<lbrakk>\<lbrakk> \<Gamma>' @ [\<gamma>] \<rbrakk>\<rbrakk>\<^sub>p\<^sub>r\<^sub>i\<^sub>m\<close>
-  by (metis symrun_interp_commute symrun_interp_decreases_add_head append_Cons append_Nil incl)
+  assumes \<open>set \<Gamma> \<subseteq> set \<Gamma>'\<close>
+    shows \<open>\<lbrakk>\<lbrakk> \<Gamma> @ [\<gamma>] \<rbrakk>\<rbrakk>\<^sub>p\<^sub>r\<^sub>i\<^sub>m \<supseteq> \<lbrakk>\<lbrakk> \<Gamma>' @ [\<gamma>] \<rbrakk>\<rbrakk>\<^sub>p\<^sub>r\<^sub>i\<^sub>m\<close>
+proof -
+  from symrun_interp_decreases_setinc[OF assms] have \<open>\<lbrakk>\<lbrakk> \<Gamma>' \<rbrakk>\<rbrakk>\<^sub>p\<^sub>r\<^sub>i\<^sub>m \<subseteq> \<lbrakk>\<lbrakk> \<Gamma> \<rbrakk>\<rbrakk>\<^sub>p\<^sub>r\<^sub>i\<^sub>m\<close> .
+  thus ?thesis by (simp add: symrun_interp_expansion dual_order.trans)
+qed
 
 lemma symrun_interp_absorb1:
-  assumes incl: \<open>set \<Gamma>\<^sub>1 \<subseteq> set \<Gamma>\<^sub>2\<close>
-  shows \<open>\<lbrakk>\<lbrakk> \<Gamma>\<^sub>1 @ \<Gamma>\<^sub>2 \<rbrakk>\<rbrakk>\<^sub>p\<^sub>r\<^sub>i\<^sub>m = \<lbrakk>\<lbrakk> \<Gamma>\<^sub>2 \<rbrakk>\<rbrakk>\<^sub>p\<^sub>r\<^sub>i\<^sub>m\<close>
-  by (simp add: Int_absorb1 symrun_interp_decreases_setinc symrun_interp_expansion incl)
+  assumes \<open>set \<Gamma>\<^sub>1 \<subseteq> set \<Gamma>\<^sub>2\<close>
+    shows \<open>\<lbrakk>\<lbrakk> \<Gamma>\<^sub>1 @ \<Gamma>\<^sub>2 \<rbrakk>\<rbrakk>\<^sub>p\<^sub>r\<^sub>i\<^sub>m = \<lbrakk>\<lbrakk> \<Gamma>\<^sub>2 \<rbrakk>\<rbrakk>\<^sub>p\<^sub>r\<^sub>i\<^sub>m\<close>
+by (simp add: Int_absorb1 symrun_interp_decreases_setinc symrun_interp_expansion assms)
 
 lemma symrun_interp_absorb2:
-  assumes incl: \<open>set \<Gamma>\<^sub>2 \<subseteq> set \<Gamma>\<^sub>1\<close>
-  shows \<open>\<lbrakk>\<lbrakk> \<Gamma>\<^sub>1 @ \<Gamma>\<^sub>2 \<rbrakk>\<rbrakk>\<^sub>p\<^sub>r\<^sub>i\<^sub>m = \<lbrakk>\<lbrakk> \<Gamma>\<^sub>1 \<rbrakk>\<rbrakk>\<^sub>p\<^sub>r\<^sub>i\<^sub>m\<close>
-  using symrun_interp_absorb1 symrun_interp_commute incl by blast
-
+  assumes \<open>set \<Gamma>\<^sub>2 \<subseteq> set \<Gamma>\<^sub>1\<close>
+    shows \<open>\<lbrakk>\<lbrakk> \<Gamma>\<^sub>1 @ \<Gamma>\<^sub>2 \<rbrakk>\<rbrakk>\<^sub>p\<^sub>r\<^sub>i\<^sub>m = \<lbrakk>\<lbrakk> \<Gamma>\<^sub>1 \<rbrakk>\<rbrakk>\<^sub>p\<^sub>r\<^sub>i\<^sub>m\<close>
+using symrun_interp_absorb1 symrun_interp_commute assms by blast
 
 end
